zoo_saturn/ws_bdeque_1: Rewrite.

theories/zoo_saturn/ws_bdeque_1.v
@@ -32,9 +32,8 @@ From zoo Require Import
 
 Implicit Types b : bool.
 Implicit Types front front_cache back : nat.
-Implicit Types l : location.
 Implicit Types id : prophet_id.
-Implicit Types v t : val.
+Implicit Types v : val.
 Implicit Types us vs ws hist priv : list val.
 Implicit Types past prophs : list prophet_identifier.(prophet_typed_type).
 Implicit Types pasts prophss : nat → list prophet_identifier.(prophet_typed_type).
@@ -81,432 +80,2135 @@ Proof.
   solve_inG.
 Qed.
 
-Section ws_bdeque_1_G.
-  Context `{ws_bdeque_1_G : WsBdeque1G Σ}.
+Module base.
+  Section ws_bdeque_1_G.
+    Context `{ws_bdeque_1_G : WsBdeque1G Σ}.
 
-  Implicit Types P : iProp Σ.
+    Implicit Types t : location.
+    Implicit Types P : iProp Σ.
 
-  Record metadata := {
-    metadata_capacity : nat ;
-    metadata_data : val ;
-    metadata_inv : namespace ;
-    metadata_prophet : prophet_id ;
-    metadata_prophet_name : prophet_multi_name ;
-    metadata_model : auth_twins_name ;
-    metadata_owner : gname ;
-    metadata_front : gname ;
-    metadata_history : gname ;
-    metadata_winner : gname ;
-  }.
-  Implicit Types γ : metadata.
+    Record ws_bdeque_1_name := {
+      ws_bdeque_1_name_capacity : nat ;
+      ws_bdeque_1_name_data : val ;
+      ws_bdeque_1_name_inv : namespace ;
+      ws_bdeque_1_name_prophet : prophet_id ;
+      ws_bdeque_1_name_prophet_name : prophet_multi_name ;
+      ws_bdeque_1_name_model : auth_twins_name ;
+      ws_bdeque_1_name_owner : gname ;
+      ws_bdeque_1_name_front : gname ;
+      ws_bdeque_1_name_history : gname ;
+      ws_bdeque_1_name_winner : gname ;
+    }.
+    Implicit Types γ : ws_bdeque_1_name.
 
-  #[local] Instance metadata_eq_dec : EqDecision metadata :=
-    ltac:(solve_decision).
-  #[local] Instance metadata_countable :
-    Countable metadata.
-  Proof.
-    solve_countable.
-  Qed.
+    #[global] Instance ws_bdeque_1_name_eq_dec : EqDecision ws_bdeque_1_name :=
+      ltac:(solve_decision).
+    #[global] Instance ws_bdeque_1_name_countable :
+      Countable ws_bdeque_1_name.
+    Proof.
+      solve_countable.
+    Qed.
 
-  #[local] Definition model₁' γ_model vs :=
-    auth_twins_twin1 _ γ_model vs.
-  #[local] Definition model₁ γ :=
-    model₁' γ.(metadata_model).
-  #[local] Definition model₂' γ_model vs :=
-    auth_twins_twin2 _ γ_model vs.
-  #[local] Definition model₂ γ :=
-    model₂' γ.(metadata_model).
+    #[local] Definition model₁' γ_model vs :=
+      auth_twins_twin1 _ γ_model vs.
+    #[local] Definition model₁ γ :=
+      model₁' γ.(ws_bdeque_1_name_model).
+    #[local] Definition model₂' γ_model vs :=
+      auth_twins_twin2 _ γ_model vs.
+    #[local] Definition model₂ γ :=
+      model₂' γ.(ws_bdeque_1_name_model).
 
-  #[local] Definition owner₁' γ_owner γ_model stable back ws : iProp Σ :=
-    twins_twin1 (twins_G := ws_bdeque_1_G_owner_G) γ_owner (DfracOwn 1) (stable, back) ∗
-    auth_twins_auth _ γ_model ws.
-  #[local] Definition owner₁ γ :=
-    owner₁' γ.(metadata_owner) γ.(metadata_model).
-  #[local] Instance : CustomIpat "owner₁" :=
-    " ( Howner₁{_{}} &
-        Hmodel_auth{_{}}
-      )
-    ".
-  #[local] Definition owner₂' γ_owner stable back :=
-    twins_twin2 (twins_G := ws_bdeque_1_G_owner_G) γ_owner (stable, back).
-  #[local] Definition owner₂ γ :=
-    owner₂' γ.(metadata_owner).
+    #[local] Definition owner₁' γ_owner γ_model stable back ws : iProp Σ :=
+      twins_twin1 (twins_G := ws_bdeque_1_G_owner_G) γ_owner (DfracOwn 1) (stable, back) ∗
+      auth_twins_auth _ γ_model ws.
+    #[local] Definition owner₁ γ :=
+      owner₁' γ.(ws_bdeque_1_name_owner) γ.(ws_bdeque_1_name_model).
+    #[local] Instance : CustomIpat "owner₁" :=
+      " ( Howner₁{_{}} &
+          Hmodel_auth{_{}}
+        )
+      ".
+    #[local] Definition owner₂' γ_owner stable back :=
+      twins_twin2 (twins_G := ws_bdeque_1_G_owner_G) γ_owner (stable, back).
+    #[local] Definition owner₂ γ :=
+      owner₂' γ.(ws_bdeque_1_name_owner).
 
-  #[local] Definition front_auth' γ_front :=
-    auth_nat_max_auth γ_front (DfracOwn 1).
-  #[local] Definition front_auth γ :=
-    front_auth' γ.(metadata_front).
-  #[local] Definition front_lb γ :=
-    auth_nat_max_lb γ.(metadata_front).
+    #[local] Definition front_auth' γ_front :=
+      auth_nat_max_auth γ_front (DfracOwn 1).
+    #[local] Definition front_auth γ :=
+      front_auth' γ.(ws_bdeque_1_name_front).
+    #[local] Definition front_lb γ :=
+      auth_nat_max_lb γ.(ws_bdeque_1_name_front).
 
-  #[local] Definition history_auth' γ_history :=
-    mono_list_auth γ_history (DfracOwn 1).
-  #[local] Definition history_auth γ :=
-    history_auth' γ.(metadata_history).
-  #[local] Definition history_at γ :=
-    mono_list_at γ.(metadata_history).
+    #[local] Definition history_auth' γ_history :=
+      mono_list_auth γ_history (DfracOwn 1).
+    #[local] Definition history_auth γ :=
+      history_auth' γ.(ws_bdeque_1_name_history).
+    #[local] Definition history_at γ :=
+      mono_list_at γ.(ws_bdeque_1_name_history).
 
-  #[local] Definition winner_pop' γ_winner front P : iProp Σ :=
-    twins_twin1 γ_winner (DfracOwn 1) (front, Next P).
-  #[local] Definition winner_pop γ :=
-    winner_pop' γ.(metadata_winner).
-  #[local] Definition winner_steal' γ_winner front P :=
-    twins_twin2 γ_winner (front, Next P).
-  #[local] Definition winner_steal γ :=
-    winner_steal' γ.(metadata_winner).
-  #[local] Definition winner γ : iProp Σ :=
-    ∃ front P1 P2,
-    winner_pop γ front P1 ∗
-    winner_steal γ front P2.
-  #[local] Instance : CustomIpat "winner" :=
-    " ( %front_winner &
-        %P_winner_1 &
-        %P_winner_2 &
-        Hwinner_pop{_{}} &
-        Hwinner_steal{_{}}
-      )
-    ".
+    #[local] Definition winner_pop' γ_winner front P : iProp Σ :=
+      twins_twin1 γ_winner (DfracOwn 1) (front, Next P).
+    #[local] Definition winner_pop γ :=
+      winner_pop' γ.(ws_bdeque_1_name_winner).
+    #[local] Definition winner_steal' γ_winner front P :=
+      twins_twin2 γ_winner (front, Next P).
+    #[local] Definition winner_steal γ :=
+      winner_steal' γ.(ws_bdeque_1_name_winner).
+    #[local] Definition winner γ : iProp Σ :=
+      ∃ front P1 P2,
+      winner_pop γ front P1 ∗
+      winner_steal γ front P2.
+    #[local] Instance : CustomIpat "winner" :=
+      " ( %front_winner &
+          %P_winner_1 &
+          %P_winner_2 &
+          Hwinner_pop{_{}} &
+          Hwinner_steal{_{}}
+        )
+      ".
 
-  #[local] Definition winner_au γ front P : iProp Σ :=
-    AU <{
-      ∃∃ vs,
-      model₁ γ vs
-    }> @ ⊤ ∖ ↑γ.(metadata_inv), ∅ <{
-      ∀∀ v vs',
-      ⌜vs = v :: vs'⌝ ∗
-      model₁ γ vs' ∗
-      history_at γ front v
-    , COMM
-      P
-    }>.
-  #[local] Definition winner_pending_1 γ front P id : iProp Σ :=
-    winner_steal γ front P ∗
-    identifier_model' id ∗
-    winner_au γ front P.
-  #[local] Instance : CustomIpat "winner_pending_1" :=
-    " ( Hwinner_steal{_{!}} &
-        Hid{_{!}} &
-        HP
-      )
-    ".
-  #[local] Definition winner_pending_2 γ front id : iProp Σ :=
-    ∃ P,
-    winner_pending_1 γ front P id.
-  #[local] Instance : CustomIpat "winner_pending_2" :=
-    " ( %P{} &
-        (:winner_pending_1)
-      )
-    ".
-  #[local] Definition winner_linearized γ front P : iProp Σ :=
-    winner_steal γ front P ∗
-    P.
-  #[local] Instance : CustomIpat "winner_linearized" :=
-    " ( Hwinner_steal{_{!}} &
-        HP
-      )
-    ".
+    #[local] Definition winner_au γ front P : iProp Σ :=
+      AU <{
+        ∃∃ vs,
+        model₁ γ vs
+      }> @ ⊤ ∖ ↑γ.(ws_bdeque_1_name_inv), ∅ <{
+        ∀∀ v vs',
+        ⌜vs = v :: vs'⌝ ∗
+        model₁ γ vs' ∗
+        history_at γ front v
+      , COMM
+        P
+      }>.
+    #[local] Definition winner_pending_1 γ front P id : iProp Σ :=
+      winner_steal γ front P ∗
+      identifier_model' id ∗
+      winner_au γ front P.
+    #[local] Instance : CustomIpat "winner_pending_1" :=
+      " ( Hwinner_steal{_{!}} &
+          Hid{_{!}} &
+          HP
+        )
+      ".
+    #[local] Definition winner_pending_2 γ front id : iProp Σ :=
+      ∃ P,
+      winner_pending_1 γ front P id.
+    #[local] Instance : CustomIpat "winner_pending_2" :=
+      " ( %P{} &
+          (:winner_pending_1)
+        )
+      ".
+    #[local] Definition winner_linearized γ front P : iProp Σ :=
+      winner_steal γ front P ∗
+      P.
+    #[local] Instance : CustomIpat "winner_linearized" :=
+      " ( Hwinner_steal{_{!}} &
+          HP
+        )
+      ".
 
-  #[local] Definition inv_state_empty γ stable front back hist : iProp Σ :=
-    ⌜stable = Stable⌝ ∗
-    ⌜front = back⌝ ∗
-    ⌜length hist = front⌝ ∗
-    winner γ.
-  #[local] Instance : CustomIpat "inv_state_empty" :=
-    " ( { {lazy}{>}%
-        ; {lazy}%
-        ; {>}->
-        ; ->
-        } &
-        {>;}-> &
-        {>;}%Hhist{} &
-        Hwinner
-      )
-    ".
-  #[local] Definition inv_state_nonempty γ stable front back hist vs prophs : iProp Σ :=
-    ⌜stable = Stable⌝ ∗
-    ⌜front < back⌝ ∗
-    ⌜length hist = S front⌝ ∗
-    history_at γ front (hd inhabitant vs) ∗
-    ( winner γ
-    ∨ match prophs with
+    #[local] Definition inv_state_empty γ stable front back hist : iProp Σ :=
+      ⌜stable = Stable⌝ ∗
+      ⌜front = back⌝ ∗
+      ⌜length hist = front⌝ ∗
+      winner γ.
+    #[local] Instance : CustomIpat "inv_state_empty" :=
+      " ( { {lazy}{>}%
+          ; {lazy}%
+          ; {>}->
+          ; ->
+          } &
+          {>;}-> &
+          {>;}%Hhist{} &
+          Hwinner
+        )
+      ".
+    #[local] Definition inv_state_nonempty γ stable front back hist vs prophs : iProp Σ :=
+      ⌜stable = Stable⌝ ∗
+      ⌜front < back⌝ ∗
+      ⌜length hist = S front⌝ ∗
+      history_at γ front (hd inhabitant vs) ∗
+      ( winner γ
+      ∨ match prophs with
+        | [] =>
+            False
+        | id :: _ =>
+            winner_pending_2 γ front id
+        end
+      ).
+    #[local] Instance : CustomIpat "inv_state_nonempty" :=
+      " ( { {lazy}{>}%
+          ; {lazy}%
+          ; {>}->
+          ; ->
+          } &
+          {>;}% &
+          {>;}%Hhist{} &
+          #Hhistory_at_front{} &
+          Hwinner
+        )
+      ".
+    #[local] Definition inv_state_nonempty_steal γ state stable front back hist vs prophs P : iProp Σ :=
+      ⌜state = Nonempty⌝ ∗
+      ⌜stable = Stable⌝ ∗
+      ⌜front < back⌝ ∗
+      ⌜length hist = S front⌝ ∗
+      history_at γ front (hd inhabitant vs) ∗
+      match prophs with
       | [] =>
           False
       | id :: _ =>
-          winner_pending_2 γ front id
-      end
-    ).
-  #[local] Instance : CustomIpat "inv_state_nonempty" :=
-    " ( { {lazy}{>}%
-        ; {lazy}%
-        ; {>}->
-        ; ->
-        } &
-        {>;}% &
-        {>;}%Hhist{} &
-        #Hhistory_at_front{} &
-        Hwinner
-      )
-    ".
-  #[local] Definition inv_state_nonempty_steal γ state stable front back hist vs prophs P : iProp Σ :=
-    ⌜state = Nonempty⌝ ∗
-    ⌜stable = Stable⌝ ∗
-    ⌜front < back⌝ ∗
-    ⌜length hist = S front⌝ ∗
-    history_at γ front (hd inhabitant vs) ∗
-    match prophs with
-    | [] =>
-        False
-    | id :: _ =>
-        winner_pending_1 γ front P id
-    end.
-  #[local] Instance : CustomIpat "inv_state_nonempty_steal" :=
-    " ( {>;}-> &
-        { {lazy}{>}%
-        ; {lazy}%
-        ; {>}->
-        ; ->
-        } &
-        {>;}% &
-        {>;}%Hhist{} &
-        #Hhistory_at_front{} &
-        Hwinner
-      )
-    ".
-  #[local] Definition inv_state_emptyish γ stable front back hist priv : iProp Σ :=
-    ∃ P,
-    ⌜stable = Unstable⌝ ∗
-    ⌜front = back⌝ ∗
-    ⌜length hist = S front⌝ ∗
-    history_at γ front (hd inhabitant priv) ∗
-    ( winner_pop γ front P
-    ∨ winner_linearized γ front P
-    ).
-  #[local] Instance : CustomIpat "inv_state_emptyish" :=
-    " ( %P_ &
-        { {lazy}{>}%
-        ; {lazy}%
-        ; {>}->
-        ; ->
-        } &
-        {>;}-> &
-        {>;}%Hhist{} &
-        #Hhistory_at_front{} &
-        Hwinner
-      )
-    ".
-  #[local] Definition inv_state_emptyish_pop γ state stable front back hist priv P : iProp Σ :=
-    ⌜state = Emptyish⌝ ∗
-    ⌜stable = Unstable⌝ ∗
-    ⌜front = back⌝ ∗
-    ⌜length hist = S front⌝ ∗
-    history_at γ front (hd inhabitant priv) ∗
-    winner_pop γ front P.
-  #[local] Instance : CustomIpat "inv_state_emptyish_pop" :=
-    " ( {>;}-> &
-        { {lazy}{>}%
-        ; {lazy}%
-        ; {>}->
-        ; ->
-        } &
-        {>;}-> &
-        {>;}%Hhist{} &
-        #Hhistory_at_front{} &
-        Hwinner_pop
-      )
-    ".
-  #[local] Definition inv_state_emptyish_steal γ state stable front back hist priv P : iProp Σ :=
-    ⌜state = Emptyish⌝ ∗
-    ⌜stable = Unstable⌝ ∗
-    ⌜front = back⌝ ∗
-    ⌜length hist = S front⌝ ∗
-    history_at γ front (hd inhabitant priv) ∗
-    winner_linearized γ front P.
-  #[local] Instance : CustomIpat "inv_state_emptyish_steal" :=
-    " ( {>;}-> &
-        { {lazy}{>}%
-        ; {lazy}%
-        ; {>}->
-        ; ->
-        } &
-        {>;}-> &
-        {>;}%Hhist{} &
-        #Hhistory_at_front{} &
-        (:winner_linearized)
-      )
-    ".
-  #[local] Definition inv_state_superempty γ stable front back hist : iProp Σ :=
-    ⌜stable = Unstable⌝ ∗
-    ⌜front = S back⌝ ∗
-    ⌜length hist = front⌝ ∗
-    winner γ.
-  #[local] Instance : CustomIpat "inv_state_superempty" :=
-    " ( { {lazy}{>}%
-        ; {lazy}%
-        ; {>}->
-        ; ->
-        } &
-        {>;}-> &
-        {>;}%Hhist{} &
-        Hwinner
-      )
-    ".
-  #[local] Definition inv_state γ state stable front back hist vs priv prophs : iProp Σ :=
-    match state with
-    | Empty =>
-        inv_state_empty γ stable front back hist
-    | Nonempty =>
-        inv_state_nonempty γ stable front back hist vs prophs
-    | Emptyish =>
-        inv_state_emptyish γ stable front back hist priv
-    | Superempty =>
-        inv_state_superempty γ stable front back hist
-    end.
+          winner_pending_1 γ front P id
+      end.
+    #[local] Instance : CustomIpat "inv_state_nonempty_steal" :=
+      " ( {>;}-> &
+          { {lazy}{>}%
+          ; {lazy}%
+          ; {>}->
+          ; ->
+          } &
+          {>;}% &
+          {>;}%Hhist{} &
+          #Hhistory_at_front{} &
+          Hwinner
+        )
+      ".
+    #[local] Definition inv_state_emptyish γ stable front back hist priv : iProp Σ :=
+      ∃ P,
+      ⌜stable = Unstable⌝ ∗
+      ⌜front = back⌝ ∗
+      ⌜length hist = S front⌝ ∗
+      history_at γ front (hd inhabitant priv) ∗
+      ( winner_pop γ front P
+      ∨ winner_linearized γ front P
+      ).
+    #[local] Instance : CustomIpat "inv_state_emptyish" :=
+      " ( %P_ &
+          { {lazy}{>}%
+          ; {lazy}%
+          ; {>}->
+          ; ->
+          } &
+          {>;}-> &
+          {>;}%Hhist{} &
+          #Hhistory_at_front{} &
+          Hwinner
+        )
+      ".
+    #[local] Definition inv_state_emptyish_pop γ state stable front back hist priv P : iProp Σ :=
+      ⌜state = Emptyish⌝ ∗
+      ⌜stable = Unstable⌝ ∗
+      ⌜front = back⌝ ∗
+      ⌜length hist = S front⌝ ∗
+      history_at γ front (hd inhabitant priv) ∗
+      winner_pop γ front P.
+    #[local] Instance : CustomIpat "inv_state_emptyish_pop" :=
+      " ( {>;}-> &
+          { {lazy}{>}%
+          ; {lazy}%
+          ; {>}->
+          ; ->
+          } &
+          {>;}-> &
+          {>;}%Hhist{} &
+          #Hhistory_at_front{} &
+          Hwinner_pop
+        )
+      ".
+    #[local] Definition inv_state_emptyish_steal γ state stable front back hist priv P : iProp Σ :=
+      ⌜state = Emptyish⌝ ∗
+      ⌜stable = Unstable⌝ ∗
+      ⌜front = back⌝ ∗
+      ⌜length hist = S front⌝ ∗
+      history_at γ front (hd inhabitant priv) ∗
+      winner_linearized γ front P.
+    #[local] Instance : CustomIpat "inv_state_emptyish_steal" :=
+      " ( {>;}-> &
+          { {lazy}{>}%
+          ; {lazy}%
+          ; {>}->
+          ; ->
+          } &
+          {>;}-> &
+          {>;}%Hhist{} &
+          #Hhistory_at_front{} &
+          (:winner_linearized)
+        )
+      ".
+    #[local] Definition inv_state_superempty γ stable front back hist : iProp Σ :=
+      ⌜stable = Unstable⌝ ∗
+      ⌜front = S back⌝ ∗
+      ⌜length hist = front⌝ ∗
+      winner γ.
+    #[local] Instance : CustomIpat "inv_state_superempty" :=
+      " ( { {lazy}{>}%
+          ; {lazy}%
+          ; {>}->
+          ; ->
+          } &
+          {>;}-> &
+          {>;}%Hhist{} &
+          Hwinner
+        )
+      ".
+    #[local] Definition inv_state γ state stable front back hist vs priv prophs : iProp Σ :=
+      match state with
+      | Empty =>
+          inv_state_empty γ stable front back hist
+      | Nonempty =>
+          inv_state_nonempty γ stable front back hist vs prophs
+      | Emptyish =>
+          inv_state_emptyish γ stable front back hist priv
+      | Superempty =>
+          inv_state_superempty γ stable front back hist
+      end.
 
-  #[local] Definition inv_inner l γ : iProp Σ :=
-    ∃ state stable front back hist vs priv pasts prophss,
-    l.[front] ↦ #front ∗
-    l.[back] ↦ #back ∗
-    owner₂ γ stable back ∗
-    front_auth γ front ∗
-    ⌜0 < front⌝ ∗
-    model₂ γ vs ∗
-    ⌜length vs = back - front⌝ ∗
-    array_cslice γ.(metadata_data) γ.(metadata_capacity) front (DfracOwn (1/2)) (vs ++ priv) ∗
-    ⌜(length vs + length priv)%nat = γ.(metadata_capacity)⌝ ∗
-    history_auth γ hist ∗
-    prophet_multi_model prophet_identifier γ.(metadata_prophet) γ.(metadata_prophet_name) pasts prophss ∗
-    ⌜∀ i, front ≤ i → pasts i = []⌝ ∗
-    inv_state γ state stable front back hist vs priv (prophss front).
-  #[local] Instance : CustomIpat "inv_inner" :=
-    " ( %state{} &
-        %stable{} &
-        %front{} &
-        %back{} &
-        %hist{} &
-        %vs{} &
-        %priv{} &
-        %pasts{} &
-        %prophss{} &
-        >Hl_front &
-        >Hl_back &
-        >Howner₂ &
-        >Hfront_auth &
-        >%Hfront{} &
-        >Hmodel₂ &
-        >%Hvs{} &
-        >Hdata_cslice₁ &
-        >%Hdata{} &
-        >Hhistory_auth &
-        >Hprophet_model &
-        >%Hpasts{} &
-        Hstate
-      )
-    ".
-  #[local] Definition inv' l γ : iProp Σ :=
-    ⌜0 < γ.(metadata_capacity)⌝ ∗
-    l.[capacity] ↦□ #γ.(metadata_capacity) ∗
-    l.[data] ↦□ γ.(metadata_data) ∗
-    l.[proph] ↦□ #γ.(metadata_prophet) ∗
-    inv γ.(metadata_inv) (inv_inner l γ).
-  #[local] Instance : CustomIpat "inv'" :=
-    " ( %Hcapacity &
-        #Hl_capacity &
-        #Hl_data &
-        #Hl_proph &
-        #Hinv
-      )
-    ".
+    #[local] Definition inv_inner t γ : iProp Σ :=
+      ∃ state stable front back hist vs priv pasts prophss,
+      t.[front] ↦ #front ∗
+      t.[back] ↦ #back ∗
+      owner₂ γ stable back ∗
+      front_auth γ front ∗
+      ⌜0 < front⌝ ∗
+      model₂ γ vs ∗
+      ⌜length vs = back - front⌝ ∗
+      array_cslice γ.(ws_bdeque_1_name_data) γ.(ws_bdeque_1_name_capacity) front (DfracOwn (1/2)) (vs ++ priv) ∗
+      ⌜(length vs + length priv)%nat = γ.(ws_bdeque_1_name_capacity)⌝ ∗
+      history_auth γ hist ∗
+      prophet_multi_model prophet_identifier γ.(ws_bdeque_1_name_prophet) γ.(ws_bdeque_1_name_prophet_name) pasts prophss ∗
+      ⌜∀ i, front ≤ i → pasts i = []⌝ ∗
+      inv_state γ state stable front back hist vs priv (prophss front).
+    #[local] Instance : CustomIpat "inv_inner" :=
+      " ( %state{} &
+          %stable{} &
+          %front{} &
+          %back{} &
+          %hist{} &
+          %vs{} &
+          %priv{} &
+          %pasts{} &
+          %prophss{} &
+          >Ht_front &
+          >Ht_back &
+          >Howner₂ &
+          >Hfront_auth &
+          >%Hfront{} &
+          >Hmodel₂ &
+          >%Hvs{} &
+          >Hdata_cslice₁ &
+          >%Hdata{} &
+          >Hhistory_auth &
+          >Hprophet_model &
+          >%Hpasts{} &
+          Hstate
+        )
+      ".
+    #[local] Definition inv' t γ : iProp Σ :=
+      ⌜0 < γ.(ws_bdeque_1_name_capacity)⌝ ∗
+      t.[capacity] ↦□ #γ.(ws_bdeque_1_name_capacity) ∗
+      t.[data] ↦□ γ.(ws_bdeque_1_name_data) ∗
+      t.[proph] ↦□ #γ.(ws_bdeque_1_name_prophet) ∗
+      inv γ.(ws_bdeque_1_name_inv) (inv_inner t γ).
+    #[local] Instance : CustomIpat "inv'" :=
+      " ( %Hcapacity &
+          #Ht_capacity &
+          #Ht_data &
+          #Ht_proph &
+          #Hinv
+        )
+      ".
+    Definition ws_bdeque_1_inv t γ ι cap : iProp Σ :=
+      ⌜ι = γ.(ws_bdeque_1_name_inv)⌝ ∗
+      ⌜cap = γ.(ws_bdeque_1_name_capacity)⌝ ∗
+      inv' t γ.
+    #[local] Instance : CustomIpat "inv" :=
+      " ( -> &
+          -> &
+          (:inv')
+        )
+      ".
+
+    Definition ws_bdeque_1_model γ vs : iProp Σ :=
+      model₁ γ vs ∗
+      ⌜length vs ≤ γ.(ws_bdeque_1_name_capacity)⌝.
+    #[local] Instance : CustomIpat "model" :=
+      " ( Hmodel₁{_{}} &
+          %Hvs{}
+        )
+      ".
+
+    Inductive owner_flag :=
+      | OwnerNormal
+      | OwnerPop.
+    #[local] Definition owner_1 flag t γ stable back ws front_cache i us : iProp Σ :=
+      owner₁ γ stable back ws ∗
+      t.[front_cache] ↦ #front_cache ∗
+      front_lb γ front_cache ∗
+      ⌜(if flag is OwnerPop then S back else back) ≤ front_cache + γ.(ws_bdeque_1_name_capacity)⌝ ∗
+      array_cslice γ.(ws_bdeque_1_name_data) γ.(ws_bdeque_1_name_capacity) i (DfracOwn (1/2)) us ∗
+      ⌜length us = γ.(ws_bdeque_1_name_capacity)⌝.
+    #[local] Instance : CustomIpat "owner_1" :=
+      " ( Howner₁{_{}} &
+          Ht_front_cache{_{}} &
+          { {!} _
+          ; #Hfront_lb_cache_{}
+          ; #Hfront_lb_cache
+          } &
+          { {!} _
+          ; %Hfront_cache_{}
+          ; %Hfront_cache
+          } &
+          Hdata_cslice₂{_{}} &
+          { {!} _
+          ; %Hus{}
+          ; %Hus
+          }
+        )
+      ".
+    #[local] Definition owner_2 :=
+      owner_1 OwnerNormal.
+    #[local] Instance : CustomIpat "owner_2" :=
+      "(:owner_1)".
+    Definition ws_bdeque_1_owner t γ ws : iProp Σ :=
+      ∃ back front_cache i us,
+      owner_2 t γ Stable back ws front_cache i us.
+    #[local] Instance : CustomIpat "owner" :=
+      " ( %back{} &
+          %front_cache{_{}} &
+          %i{} &
+          %us{} &
+          Howner{_{}}
+        )
+      ".
+
+    #[global] Instance ws_bdeque_1_model_timeless γ vs :
+      Timeless (ws_bdeque_1_model γ vs).
+    Proof.
+      apply _.
+    Qed.
+    #[global] Instance ws_bdeque_1_owner_timeless t γ ws :
+      Timeless (ws_bdeque_1_owner t γ ws).
+    Proof.
+      apply _.
+    Qed.
+
+    #[global] Instance ws_bdeque_1_inv_persistent t γ ι cap :
+      Persistent (ws_bdeque_1_inv t γ ι cap).
+    Proof.
+      apply _.
+    Qed.
+
+    #[local] Lemma model_owner_alloc :
+      ⊢ |==>
+        ∃ γ_model γ_owner,
+        model₁' γ_model [] ∗
+        model₂' γ_model [] ∗
+        owner₁' γ_owner γ_model Stable 1 [] ∗
+        owner₂' γ_owner Stable 1.
+    Proof.
+      iMod (auth_twins_alloc _ (auth_twins_G := ws_bdeque_1_G_model_G)) as "(%γ_model & Hmodel_auth & Hmodel₁ & Hmodel₂)".
+      iMod (twins_alloc' (twins_G := ws_bdeque_1_G_owner_G)) as "(%γ_owner & Howner₁ & Howner₂)".
+      iFrameSteps.
+    Qed.
+    #[local] Lemma model₁_valid γ stable back ws vs :
+      owner₁ γ stable back ws -∗
+      model₁ γ vs -∗
+      ⌜vs `suffix_of` ws⌝.
+    Proof.
+      iIntros "(:owner₁) Hmodel₁".
+      iDestruct (auth_twins_valid_1 with "Hmodel_auth Hmodel₁") as %H.
+      rewrite preorder_rtc in H. iSteps.
+    Qed.
+    #[local] Lemma model₁_exclusive γ vs1 vs2 :
+      model₁ γ vs1 -∗
+      model₁ γ vs2 -∗
+      False.
+    Proof.
+      apply auth_twins_twin1_exclusive.
+    Qed.
+    #[local] Lemma model_agree γ vs1 vs2 :
+      model₁ γ vs1 -∗
+      model₂ γ vs2 -∗
+      ⌜vs1 = vs2⌝.
+    Proof.
+      apply: auth_twins_agree_L.
+    Qed.
+    #[local] Lemma model_owner₁_agree γ stable back ws vs1 vs2 :
+      owner₁ γ stable back ws -∗
+      model₁ γ vs1 -∗
+      model₂ γ vs2 -∗
+        ⌜vs1 `suffix_of` ws⌝ ∗
+        ⌜vs1 = vs2⌝.
+    Proof.
+      iIntros "Howner₁ Hmodel₁ Hmodel₂".
+      iDestruct (model₁_valid with "Howner₁ Hmodel₁") as %Hsuffix.
+      iDestruct (model_agree with "Hmodel₁ Hmodel₂") as %->.
+      iSteps.
+    Qed.
+    #[local] Lemma model_empty {γ stable back ws vs1 vs2} :
+      owner₁ γ stable back ws -∗
+      model₁ γ vs1 -∗
+      model₂ γ vs2 ==∗
+        owner₁ γ stable back [] ∗
+        model₁ γ [] ∗
+        model₂ γ [].
+    Proof.
+      iIntros "(:owner₁) Hmodel₁ Hmodel₂".
+      iMod (auth_twins_update_auth with "Hmodel_auth Hmodel₁ Hmodel₂") as "(Hmodel_auth & Hmodel₁ & Hmodel₂)".
+      iSteps.
+    Qed.
+    #[local] Lemma model_push {γ stable back ws vs1 vs2} v :
+      owner₁ γ stable back ws -∗
+      model₁ γ vs1 -∗
+      model₂ γ vs2 ==∗
+        owner₁ γ stable back (vs1 ++ [v]) ∗
+        model₁ γ (vs1 ++ [v]) ∗
+        model₂ γ (vs1 ++ [v]).
+    Proof.
+      iIntros "(:owner₁) Hmodel₁ Hmodel₂".
+      iMod (auth_twins_update_auth with "Hmodel_auth Hmodel₁ Hmodel₂") as "(Hmodel_auth & Hmodel₁ & Hmodel₂)".
+      iSteps.
+    Qed.
+    #[local] Lemma model_steal γ vs1 vs2 :
+      model₁ γ vs1 -∗
+      model₂ γ vs2 ==∗
+        model₁ γ (tail vs1) ∗
+        model₂ γ (tail vs1).
+    Proof.
+      apply: auth_twins_update_twins_L.
+      rewrite preorder_rtc. apply suffix_tail. done.
+    Qed.
+    #[local] Lemma model_pop γ stable back ws vs1 vs2 :
+      owner₁ γ stable back ws -∗
+      model₁ γ vs1 -∗
+      model₂ γ vs2 ==∗
+        owner₁ γ stable back (removelast vs1) ∗
+        model₁ γ (removelast vs1) ∗
+        model₂ γ (removelast vs1).
+    Proof.
+      iIntros "(:owner₁) Hmodel₁ Hmodel₂".
+      iMod (auth_twins_update_auth with "Hmodel_auth Hmodel₁ Hmodel₂") as "(Hmodel_auth & Hmodel₁ & Hmodel₂)".
+      iSteps.
+    Qed.
+    #[local] Lemma model_pop' γ stable back ws vs1 v vs2 :
+      owner₁ γ stable back ws -∗
+      model₁ γ (vs1 ++ [v]) -∗
+      model₂ γ vs2 ==∗
+        owner₁ γ stable back vs1 ∗
+        model₁ γ vs1 ∗
+        model₂ γ vs1.
+    Proof.
+      rewrite -{2 3 4}(removelast_last vs1 v).
+      apply model_pop.
+    Qed.
+
+    #[local] Lemma owner₁_exclusive γ stable1 back1 ws1 stable2 back2 ws2 :
+      owner₁ γ stable1 back1 ws1 -∗
+      owner₁ γ stable2 back2 ws2 -∗
+      False.
+    Proof.
+      iIntros "(:owner₁ =1) (:owner₁ =2)".
+      iApply (twins_twin1_exclusive with "Howner₁_1 Howner₁_2").
+    Qed.
+    #[local] Lemma owner_agree γ stable1 back1 ws stable2 back2 :
+      owner₁ γ stable1 back1 ws -∗
+      owner₂ γ stable2 back2 -∗
+        ⌜stable1 = stable2⌝ ∗
+        ⌜back1 = back2⌝.
+    Proof.
+      iIntros "(:owner₁) Howner₂".
+      iDestruct (twins_agree_L with "Howner₁ Howner₂") as %[= <- <-].
+      iSteps.
+    Qed.
+    #[local] Lemma owner₁_update γ stable back ws vs :
+      owner₁ γ stable back ws -∗
+      model₁ γ vs -∗
+      model₂ γ vs ==∗
+        owner₁ γ stable back vs ∗
+        model₁ γ vs ∗
+        model₂ γ vs.
+    Proof.
+      iIntros "(:owner₁) Hmodel₁ Hmodel₂".
+      iMod (auth_twins_update_auth with "Hmodel_auth Hmodel₁ Hmodel₂") as "($ & $ & $)".
+      iSteps.
+    Qed.
+    #[local] Lemma owner_update {γ stable1 back1 ws stable2 back2} stable back :
+      owner₁ γ stable1 back1 ws -∗
+      owner₂ γ stable2 back2 ==∗
+        owner₁ γ stable back ws ∗
+        owner₂ γ stable back.
+    Proof.
+      iIntros "(:owner₁) Howner₂".
+      iMod (twins_update with "Howner₁ Howner₂") as "(Howner₁ & Howner₂)".
+      iSteps.
+    Qed.
+
+    #[local] Lemma front_alloc :
+      ⊢ |==>
+        ∃ γ_front,
+        front_auth' γ_front 1.
+    Proof.
+      apply auth_nat_max_alloc.
+    Qed.
+    #[local] Lemma front_lb_get γ front :
+      front_auth γ front ⊢
+      front_lb γ front.
+    Proof.
+      apply auth_nat_max_lb_get.
+    Qed.
+    #[local] Lemma front_lb_le {γ front} front' :
+      front' ≤ front →
+      front_lb γ front ⊢
+      front_lb γ front'.
+    Proof.
+      apply auth_nat_max_lb_le.
+    Qed.
+    #[local] Lemma front_lb_valid γ front1 front2 :
+      front_auth γ front1 -∗
+      front_lb γ front2 -∗
+      ⌜front2 ≤ front1⌝.
+    Proof.
+      apply auth_nat_max_lb_valid.
+    Qed.
+    #[local] Lemma front_update γ front :
+      front_auth γ front ⊢ |==>
+      front_auth γ (S front).
+    Proof.
+      apply auth_nat_max_update; first lia.
+    Qed.
+
+    #[local] Lemma history_alloc :
+      ⊢ |==>
+        ∃ γ_hist,
+        history_auth' γ_hist [()%V].
+    Proof.
+      apply mono_list_alloc.
+    Qed.
+    #[local] Lemma history_at_get {γ hist v} i :
+      i = length hist →
+      history_auth γ (hist ++ [v]) ⊢
+      history_at γ i v.
+    Proof.
+      intros ->.
+      apply mono_list_at_get, list_lookup_middle. done.
+    Qed.
+    #[local] Lemma history_at_lookup γ hist i v :
+      history_auth γ hist -∗
+      history_at γ i v -∗
+      ⌜hist !! i = Some v⌝.
+    Proof.
+      apply mono_list_at_valid.
+    Qed.
+    #[local] Lemma history_at_agree γ i v1 v2 :
+      history_at γ i v1 -∗
+      history_at γ i v2 -∗
+      ⌜v1 = v2⌝.
+    Proof.
+      apply mono_list_at_agree.
+    Qed.
+    #[local] Lemma history_update {γ hist} i v :
+      i = length hist →
+      history_auth γ hist ⊢ |==>
+        history_auth γ (hist ++ [v]) ∗
+        history_at γ i v.
+    Proof.
+      iIntros (->) "Hauth".
+      iMod (mono_list_update_snoc with "Hauth") as "Hauth".
+      iDestruct (history_at_get with "Hauth") as "#Hat"; first done.
+      iSteps.
+    Qed.
+
+    #[local] Lemma winner_alloc :
+      ⊢ |==>
+        ∃ γ_winner,
+        winner_pop' γ_winner 1 True ∗
+        winner_steal' γ_winner 1 True.
+    Proof.
+      apply twins_alloc'.
+    Qed.
+    #[local] Lemma winner_pop_exclusive γ front1 P1 front2 P2 :
+      winner_pop γ front1 P1 -∗
+      winner_pop γ front2 P2 -∗
+      False.
+    Proof.
+      apply twins_twin1_exclusive.
+    Qed.
+    #[local] Lemma winner_pop_exclusive' γ front P :
+      winner_pop γ front P -∗
+      winner γ -∗
+      False.
+    Proof.
+      iIntros "Hwinner_pop_1 (:winner =2)".
+      iApply (winner_pop_exclusive with "Hwinner_pop_1 Hwinner_pop_2").
+    Qed.
+    #[local] Lemma winner_steal_exclusive γ front1 P1 front2 P2 :
+      winner_steal γ front1 P1 -∗
+      winner_steal γ front2 P2 -∗
+      False.
+    Proof.
+      apply twins_twin2_exclusive.
+    Qed.
+    #[local] Lemma winner_steal_exclusive' γ front P :
+      winner_steal γ front P -∗
+      winner γ -∗
+      False.
+    Proof.
+      iIntros "Hwinner_steal_1 (:winner =2)".
+      iApply (winner_steal_exclusive with "Hwinner_steal_1 Hwinner_steal_2").
+    Qed.
+    #[local] Lemma winner_agree γ front1 P1 front2 P2 :
+      winner_pop γ front1 P1 -∗
+      winner_steal γ front2 P2 -∗
+        ⌜front1 = front2⌝ ∗
+        ▷ (P1 ≡ P2).
+    Proof.
+      iIntros "Hwinner_pop Hwinner_steal".
+      iDestruct (twins_agree with "Hwinner_pop Hwinner_steal") as "#Heq".
+      rewrite prod_equivI /= discrete_eq_1.
+      iDestruct "Heq" as "($ & $)".
+    Qed.
+    #[local] Lemma winner_update {γ front1 P1 front2 P2} front P :
+      winner_pop γ front1 P1 -∗
+      winner_steal γ front2 P2 ==∗
+        winner_pop γ front P ∗
+        winner_steal γ front P.
+    Proof.
+      apply twins_update.
+    Qed.
+
+    Opaque owner₁'.
+
+    Lemma ws_bdeque_1_model_valid t γ ι cap vs :
+      ws_bdeque_1_inv t γ ι cap -∗
+      ws_bdeque_1_model γ vs -∗
+      ⌜length vs ≤ cap⌝.
+    Proof.
+      iSteps.
+    Qed.
+    Lemma ws_bdeque_1_model_exclusive γ vs1 vs2 :
+      ws_bdeque_1_model γ vs1 -∗
+      ws_bdeque_1_model γ vs2 -∗
+      False.
+    Proof.
+      iIntros "(:model =1) (:model =2)".
+      iApply (model₁_exclusive with "Hmodel₁_1 Hmodel₁_2").
+    Qed.
+
+    #[local] Lemma owner_2_rebase {t γ stable back ws front_cache i1 us} i2 :
+      0 < γ.(ws_bdeque_1_name_capacity) →
+      owner_2 t γ stable back ws front_cache i1 us ⊢
+        ∃ us,
+        owner_2 t γ stable back ws front_cache i2 us.
+    Proof.
+      iIntros "%Hcapacity (:owner_2)".
+      iDestruct (array_cslice_rebase i2 with "Hdata_cslice₂") as "(%us' & %n & -> & Hdata_cslice₂ & _)"; [done.. |].
+      iSteps. simpl_length.
+    Qed.
+
+    Lemma ws_bdeque_1_owner_exclusive t γ ws1 ws2 :
+      ws_bdeque_1_owner t γ ws1 -∗
+      ws_bdeque_1_owner t γ ws2 -∗
+      False.
+    Proof.
+      iIntros "(:owner =1) (:owner =2)".
+      iDestruct "Howner_1" as "(:owner_2 =1)".
+      iDestruct "Howner_2" as "(:owner_2 =2)".
+      iApply (owner₁_exclusive with "Howner₁_1 Howner₁_2").
+    Qed.
+    Lemma ws_bdeque_1_owner_model t γ ws vs :
+      ws_bdeque_1_owner t γ ws -∗
+      ws_bdeque_1_model γ vs -∗
+      ⌜vs `suffix_of` ws⌝.
+    Proof.
+      iIntros "(:owner =1) (:model =2)".
+      iDestruct "Howner_1" as "(:owner_2 =1)".
+      iApply (model₁_valid with "Howner₁_1 Hmodel₁_2").
+    Qed.
+
+    #[local] Lemma inv_state_Stable γ state front back hist vs priv prophs :
+      length vs = back - front →
+      inv_state γ state Stable front back hist vs priv prophs ⊢
+        ⌜state = Empty ∨ state = Nonempty⌝ ∗
+        ⌜front ≤ back⌝.
+    Proof.
+      iIntros "%Hvs Hstate".
+      destruct state.
+      - iDestruct "Hstate" as "(:inv_state_empty lazy=)".
+        iSteps.
+      - iDestruct "Hstate" as "(:inv_state_nonempty lazy=)".
+        iSteps.
+      - iDestruct "Hstate" as "(:inv_state_emptyish lazy=)". done.
+      - iDestruct "Hstate" as "(:inv_state_superempty lazy=)". done.
+    Qed.
+    #[local] Lemma inv_state_Unstable γ state front back hist vs priv prophs :
+      inv_state γ state Unstable front back hist vs priv prophs ⊢
+        ⌜state = Emptyish ∨ state = Superempty⌝ ∗
+        ⌜front = back ∨ front = S back⌝.
+    Proof.
+      iIntros "Hstate".
+      destruct state.
+      - iDestruct "Hstate" as "(:inv_state_empty lazy=)". done.
+      - iDestruct "Hstate" as "(:inv_state_nonempty lazy=)". done.
+      - iDestruct "Hstate" as "(:inv_state_emptyish lazy=)".
+        iSteps.
+      - iDestruct "Hstate" as "(:inv_state_superempty lazy=)".
+        iSteps.
+    Qed.
+    #[local] Lemma inv_state_Nonempty γ state stable front back hist vs priv prophs :
+      front < back →
+      inv_state γ state stable front back hist vs priv prophs ⊢
+      ⌜state = Nonempty⌝.
+    Proof.
+      iIntros "% Hstate".
+      destruct state.
+      - iDestruct "Hstate" as "(:inv_state_empty)". lia.
+      - done.
+      - iDestruct "Hstate" as "(:inv_state_emptyish)". lia.
+      - iDestruct "Hstate" as "(:inv_state_superempty)". lia.
+    Qed.
+    #[local] Lemma inv_state_Superempty γ state front back hist vs priv prophs :
+      back < front →
+      inv_state γ state Unstable front back hist vs priv prophs -∗
+      ⌜state = Superempty⌝.
+    Proof.
+      iIntros "% Hstate".
+      destruct state.
+      - iDestruct "Hstate" as "(:inv_state_empty lazy=)". done.
+      - iDestruct "Hstate" as "(:inv_state_nonempty lazy=)". done.
+      - iDestruct "Hstate" as "(:inv_state_emptyish lazy=)". lia.
+      - done.
+    Qed.
+    #[local] Lemma inv_state_winner_pop γ state stable front1 back hist vs priv prophs front2 P :
+      inv_state γ state stable front1 back hist vs priv prophs -∗
+      winner_pop γ front2 P -∗
+        ∃ P_,
+        ⌜front1 = front2⌝ ∗
+        ▷ (P ≡ P_) ∗
+        ( inv_state_nonempty_steal γ state stable front2 back hist vs prophs P_
+        ∨ inv_state_emptyish_steal γ state stable front2 back hist priv P_
+        ) ∗
+        winner_pop γ front2 P.
+    Proof.
+      iIntros "Hstate Hwinner_pop".
+      destruct state.
+      - iDestruct "Hstate" as "(:inv_state_empty)".
+        iDestruct "Hwinner" as "(:winner =3)".
+        iDestruct (winner_pop_exclusive with "Hwinner_pop Hwinner_pop_3") as %[].
+      - iDestruct "Hstate" as "(:inv_state_nonempty)".
+        iDestruct "Hwinner" as "[(:winner =3) | Hwinner]".
+        + iDestruct (winner_pop_exclusive with "Hwinner_pop Hwinner_pop_3") as %[].
+        + destruct prophs as [| id prophs]; first done.
+          iDestruct "Hwinner" as "(:winner_pending_2 =_)".
+          iDestruct (winner_agree with "Hwinner_pop Hwinner_steal") as "#(<- & $)".
+          iSteps.
+      - iDestruct "Hstate" as "(:inv_state_emptyish)".
+        iDestruct "Hwinner" as "[Hwinner_pop_ | (:winner_linearized)]".
+        + iDestruct (winner_pop_exclusive with "Hwinner_pop Hwinner_pop_") as %[].
+        + iDestruct (winner_agree with "Hwinner_pop Hwinner_steal") as "#(<- & $)".
+          iSteps.
+      - iDestruct "Hstate" as "(:inv_state_superempty)".
+        iDestruct "Hwinner" as "(:winner =3)".
+        iDestruct (winner_pop_exclusive with "Hwinner_pop Hwinner_pop_3") as %[].
+    Qed.
+    #[local] Lemma inv_state_winner_steal γ state stable front1 back hist vs priv prophs front2 P :
+      inv_state γ state stable front1 back hist vs priv prophs -∗
+      winner_steal γ front2 P -∗
+        ∃ P_,
+        ⌜front1 = front2⌝ ∗
+        ▷ (P_ ≡ P) ∗
+        inv_state_emptyish_pop γ state stable front2 back hist priv P_ ∗
+        winner_steal γ front2 P.
+    Proof.
+      iIntros "Hstate Hwinner_steal".
+      destruct state.
+      - iDestruct "Hstate" as "(:inv_state_empty)".
+        iDestruct "Hwinner" as "(:winner =3)".
+        iDestruct (winner_steal_exclusive with "Hwinner_steal Hwinner_steal_3") as %[].
+      - iDestruct "Hstate" as "(:inv_state_nonempty)".
+        destruct prophs as [| id prophs].
+        + iDestruct "Hwinner" as "[(:winner =3) | []]".
+          iDestruct (winner_steal_exclusive with "Hwinner_steal Hwinner_steal_3") as %[].
+        + iDestruct "Hwinner" as "[(:winner =3) | (:winner_pending_2 =_ !=)]".
+          * iDestruct (winner_steal_exclusive with "Hwinner_steal Hwinner_steal_3") as %[].
+          * iDestruct (winner_steal_exclusive with "Hwinner_steal Hwinner_steal_") as %[].
+      - iDestruct "Hstate" as "(:inv_state_emptyish)".
+        iDestruct "Hwinner" as "[Hwinner_pop | (:winner_linearized !=)]".
+        + iDestruct (winner_agree with "Hwinner_pop Hwinner_steal") as "#(<- & $)".
+          iSteps.
+        + iDestruct (winner_steal_exclusive with "Hwinner_steal Hwinner_steal_") as %[].
+      - iDestruct "Hstate" as "(:inv_state_superempty)".
+        iDestruct "Hwinner" as "(:winner =3)".
+        iDestruct (winner_steal_exclusive with "Hwinner_steal Hwinner_steal_3") as %[].
+    Qed.
+
+    Lemma ws_bdeque_1_create_spec ι (cap : Z) :
+      (0 < cap)%Z →
+      {{{
+        True
+      }}}
+        ws_bdeque_1_create #cap
+      {{{ t γ,
+        RET #t;
+        meta_token t ⊤ ∗
+        ws_bdeque_1_inv t γ ι ₊cap ∗
+        ws_bdeque_1_model γ [] ∗
+        ws_bdeque_1_owner t γ []
+      }}}.
+    Proof.
+      iIntros "%Hcap %Φ _ HΦ".
+
+      wp_rec.
+
+      wp_apply (prophet_multi_wp_proph with "[//]") as (pid γ_prophet prophss) "Hprophet_model".
+
+      wp_apply (array_unsafe_make_spec with "[//]") as (data) "Hdata_model"; first lia.
+      iDestruct (array_model_to_cslice with "Hdata_model") as "Hdata_cslice".
+      iEval (simpl_length) in "Hdata_cslice".
+      iDestruct (array_cslice_rotation_right_0 1 with "Hdata_cslice") as "Hdata_cslice"; [simpl_length; lia.. |].
+      iEval (rewrite rotation_replicate) in "Hdata_cslice".
+      iDestruct "Hdata_cslice" as "(Hdata_cslice₁ & Hdata_cslice₂)".
+
+      wp_block t as "Hmeta" "(Ht_capacity & Ht_front & Ht_front_cache & Ht_back & Ht_data & Ht_proph & _)".
+      iMod (pointsto_persist with "Ht_capacity") as "#Ht_capacity".
+      iMod (pointsto_persist with "Ht_data") as "#Ht_data".
+      iMod (pointsto_persist with "Ht_proph") as "#Ht_proph".
+
+      iMod model_owner_alloc as "(%γ_model & %γ_owner & Hmodel₁ & Hmodel₂ & Howner₁ & Howner₂)".
+      iMod front_alloc as "(%γ_front & Hfront_auth)".
+      iMod history_alloc as "(%γ_history & Hhist_auth)".
+      iMod winner_alloc as "(%γ_winner & Hwinner_pop & Hwinner_steal)".
+
+      set γ := {|
+        ws_bdeque_1_name_capacity := ₊cap ;
+        ws_bdeque_1_name_data := data ;
+        ws_bdeque_1_name_inv := ι ;
+        ws_bdeque_1_name_prophet := pid ;
+        ws_bdeque_1_name_prophet_name := γ_prophet ;
+        ws_bdeque_1_name_model := γ_model ;
+        ws_bdeque_1_name_owner := γ_owner ;
+        ws_bdeque_1_name_front := γ_front ;
+        ws_bdeque_1_name_history := γ_history ;
+        ws_bdeque_1_name_winner := γ_winner ;
+      |}.
+
+      iDestruct (front_lb_get γ with "Hfront_auth") as "#Hfront_lb".
+
+      iApply ("HΦ" $! t γ).
+      iFrame "#∗". iSplitL.
+      - iStep 4.
+        iApply inv_alloc.
+        iExists Empty, Stable, 1, 1, [()%V], [], (replicate ₊cap ()%V), (λ _, []), prophss. iFrameSteps.
+        iPureIntro. simpl_length.
+      - iSteps.
+        iPureIntro. simpl_length.
+    Qed.
+
+    Lemma ws_bdeque_1_capacity_spec t γ ι cap :
+      {{{
+        ws_bdeque_1_inv t γ ι cap
+      }}}
+        ws_bdeque_1_capacity #t
+      {{{
+        RET #cap;
+        True
+      }}}.
+    Proof.
+      iIntros "%Φ (:inv) HΦ".
+
+      wp_rec. wp_load.
+      iSteps.
+    Qed.
+
+    #[local] Lemma front_spec t γ :
+      {{{
+        inv' t γ
+      }}}
+        (#t).{front}
+      {{{ front,
+        RET #front;
+        front_lb γ front
+      }}}.
+    Proof.
+      iIntros "%Φ (:inv') HΦ".
+
+      iInv "Hinv" as "(:inv_inner)".
+      wp_load.
+      iDestruct (front_lb_get with "Hfront_auth") as "#Hfront_lb_1".
+      iFrameSteps.
+    Qed.
+    #[local] Lemma front_spec_owner_Stable t γ back ws :
+      {{{
+        inv' t γ ∗
+        owner₁ γ Stable back ws
+      }}}
+        (#t).{front}
+      {{{ front,
+        RET #front;
+        owner₁ γ Stable back ws ∗
+        front_lb γ front ∗
+        ⌜front ≤ back⌝
+      }}}.
+    Proof.
+      iIntros "%Φ ((:inv') & Howner₁) HΦ".
+
+      iInv "Hinv" as "(:inv_inner =1)".
+      wp_load.
+      iDestruct (owner_agree with "Howner₁ Howner₂") as %(<- & <-).
+      iDestruct (front_lb_get with "Hfront_auth") as "#Hfront_lb".
+      iDestruct (inv_state_Stable with "Hstate") as "#(_ & %)"; first done.
+      iFrameSteps.
+    Qed.
+    #[local] Lemma front_spec_owner_Unstable t γ back ws :
+      {{{
+        inv' t γ ∗
+        owner₁ γ Unstable back ws
+      }}}
+        (#t).{front}
+      {{{ front,
+        RET #front;
+        owner₁ γ Unstable back ws ∗
+        front_lb γ front ∗
+        ⌜front = back ∨ front = S back⌝
+      }}}.
+    Proof.
+      iIntros "%Φ ((:inv') & Howner₁) HΦ".
+
+      iInv "Hinv" as "(:inv_inner =1)".
+      wp_load.
+      iDestruct (owner_agree with "Howner₁ Howner₂") as %(<- & <-).
+      iDestruct (front_lb_get with "Hfront_auth") as "#Hfront_lb".
+      iDestruct (inv_state_Unstable with "Hstate") as "#(_ & %)".
+      iFrameSteps.
+    Qed.
+    #[local] Lemma front_spec_Superempty t γ back ws front :
+      back < front →
+      {{{
+        inv' t γ ∗
+        owner₁ γ Unstable back ws ∗
+        front_lb γ front
+      }}}
+        (#t).{front}
+      {{{
+        RET #front;
+        owner₁ γ Unstable back ws
+      }}}.
+    Proof.
+      iIntros "% %Φ ((:inv') & Howner₁ & #Hfront_lb) HΦ".
+
+      iInv "Hinv" as "(:inv_inner =1)".
+      wp_load.
+      iDestruct (owner_agree with "Howner₁ Howner₂") as %(<- & <-).
+      iDestruct (front_lb_valid with "Hfront_auth Hfront_lb") as %?.
+      iDestruct (inv_state_Superempty with "Hstate") as %->; first lia.
+      iDestruct "Hstate" as "(:inv_state_superempty =1 lazy=)".
+      iSplitR "Howner₁ HΦ". { iExists Superempty. iFrameSteps. }
+      replace (S back) with front by lia.
+      iSteps.
+    Qed.
+    #[local] Lemma front_spec_winner_steal t γ front P :
+      {{{
+        inv' t γ ∗
+        winner_steal γ front P
+      }}}
+        (#t).{front}
+      {{{
+        RET #front;
+        winner_steal γ front P
+      }}}.
+    Proof.
+      iIntros "%Φ ((:inv') & Hwinner_steal) HΦ".
+
+      iInv "Hinv" as "(:inv_inner =1)".
+      wp_load.
+
+      iAssert ⌜front1 = front⌝%I as %->.
+      { iDestruct (inv_state_winner_steal with "Hstate Hwinner_steal") as "(%P_ & $ & _)". }
+
+      iFrameSteps.
+    Qed.
+
+    #[local] Lemma back_spec t γ stable back ws :
+      {{{
+        inv' t γ ∗
+        owner₁ γ stable back ws
+      }}}
+        (#t).{back}
+      {{{
+        RET #back;
+        owner₁ γ stable back ws
+      }}}.
+    Proof.
+      iIntros "%Φ ((:inv') & Howner₁) HΦ".
+
+      iInv "Hinv" as "(:inv_inner =1)".
+      wp_load.
+      iDestruct (owner_agree with "Howner₁ Howner₂") as "(<- & <-)".
+      iFrameSteps.
+    Qed.
+
+    #[local] Lemma set_back_spec_Superempty t γ back ws front (back' : Z) :
+      back < front →
+      back' = S back →
+      {{{
+        inv' t γ ∗
+        owner₁ γ Unstable back ws ∗
+        front_lb γ front
+      }}}
+        #t <-{back} #back'
+      {{{
+        RET ();
+        owner₁ γ Stable (S back) ws
+      }}}.
+    Proof.
+      iIntros (? ->) "%Φ ((:inv') & Howner₁ & #Hfront_lb) HΦ".
+
+      iInv "Hinv" as "(:inv_inner =1)".
+      wp_store.
+      iDestruct (owner_agree with "Howner₁ Howner₂") as %(<- & <-).
+      iMod (owner_update Stable (S back) with "Howner₁ Howner₂") as "(Howner₁ & Howner₂)".
+      iDestruct (front_lb_valid with "Hfront_auth Hfront_lb") as %?.
+      iDestruct (inv_state_Superempty with "Hstate") as %->; first lia.
+      iDestruct "Hstate" as "(:inv_state_superempty =1 lazy=)".
+      iSplitR "Howner₁ HΦ". { iExists Empty. iFrameSteps. }
+      iSteps.
+    Qed.
+
+    #[local] Lemma array_unsafe_cget_spec_loser t γ i :
+      (0 ≤ i)%Z →
+      {{{
+        inv' t γ
+      }}}
+        array_unsafe_cget γ.(ws_bdeque_1_name_data) #i
+      {{{ v,
+        RET v;
+        True
+      }}}.
+    Proof.
+      iIntros "%Hi %Φ (:inv') HΦ".
+
+      iApply wp_fupd.
+      awp_apply (array_unsafe_cget_spec_atomic_weak with "[//]") without "HΦ"; first done.
+      iInv "Hinv" as "(:inv_inner)".
+      iAaccIntro with "[$Hdata_cslice₁]".
+      { iPureIntro. simpl_length. }
+      { iIntros "(Hdata_cslice₁ & _) !>". iFrameSteps. }
+      iIntros "Hdata_cslice₁ !>".
+      iSplitL. { iFrameSteps. }
+      iIntros "%v H£ HΦ".
+      iApply (lc_fupd_elim_later with "H£ HΦ [//]").
+    Qed.
+    #[local] Lemma array_unsafe_cget_spec_winner_pop t γ front P v :
+      {{{
+        inv' t γ ∗
+        winner_pop γ front P ∗
+        history_at γ front v
+      }}}
+        array_unsafe_cget γ.(ws_bdeque_1_name_data) #front
+      {{{
+        RET v;
+        winner_pop γ front P
+      }}}.
+    Proof.
+      iIntros "%Φ ((:inv') & Hwinner_pop & #Hhistory_at) HΦ".
+
+      iApply wp_fupd.
+      awp_apply (array_unsafe_cget_spec_atomic with "[//]") without "HΦ".
+      iInv "Hinv" as "(:inv_inner =1)".
+
+      iAssert (◇ (
+        ⌜front1 = front⌝ ∗
+        ⌜hd inhabitant (vs1 ++ priv1) = v⌝
+      ))%I as "#>(-> & %Hlookup)".
+      { iDestruct (inv_state_winner_pop with "Hstate [$Hwinner_pop]") as "(%P_ & >-> & _ & [(:inv_state_nonempty_steal =1 >) | (:inv_state_emptyish_steal =1 >)] & Hwinner_pop)".
+        - iDestruct (history_at_agree with "Hhistory_at Hhistory_at_front1") as ">->".
+          rewrite hd_app //; first lia.
+        - iDestruct (history_at_agree with "Hhistory_at Hhistory_at_front1") as ">->".
+          assert (length vs1 = 0) as ->%nil_length_inv by lia.
+          iSteps.
+      }
+      apply hd_correct in Hlookup; last (simpl_length; lia).
+      rewrite head_lookup in Hlookup.
+
+      iAaccIntro with "[$Hdata_cslice₁]".
+      { rewrite Nat2Z.id Nat.sub_diag. iSteps. }
+      { iIntros "(_ & _ & Hdata_cslice₁) !>". iFrameSteps. }
+      iIntros "Hdata_cslice₁ !>".
+      iSplitR "Hwinner_pop". { iFrameSteps. }
+      iIntros "H£ HΦ".
+      iApply (lc_fupd_elim_later with "H£ HΦ Hwinner_pop").
+    Qed.
+
+    #[local] Lemma array_unsafe_cset_spec_owner t γ back ws front_cache us front v :
+      back < front + γ.(ws_bdeque_1_name_capacity) →
+      {{{
+        inv' t γ ∗
+        owner_2 t γ Stable back ws front_cache back us ∗
+        front_lb γ front
+      }}}
+        array_unsafe_cset γ.(ws_bdeque_1_name_data) #back v
+      {{{
+        RET ();
+        owner_2 t γ Stable back ws front_cache back (<[0 := v]> us)
+      }}}.
+    Proof.
+      iIntros "% %Φ ((:inv') & (:owner_2) & #Hfront_lb) HΦ".
+
+      iApply wp_fupd.
+      awp_apply (array_unsafe_cset_spec_atomic_cell with "[//]") without "HΦ".
+      iInv "Hinv" as "(:inv_inner =1)".
+      iDestruct (owner_agree with "Howner₁ Howner₂") as %(<- & <-).
+      iDestruct (front_lb_valid with "Hfront_auth Hfront_lb") as %?.
+      iDestruct (inv_state_Stable with "Hstate") as "#>(%Hstate1 & %)"; first done.
+
+      iDestruct (array_cslice_app with "Hdata_cslice₁") as "(Hdata_cslice₁_1 & Hdata_cslice₁_2)".
+      destruct (lookup_lt_is_Some_2 priv1 0) as (w & Hpriv_lookup); first lia.
+      iDestruct (array_cslice_update with "Hdata_cslice₁_2") as "(Hdata_back₁ & Hdata_cslice₁_2)"; first done.
+      replace (front1 + length vs1 + 0) with back by lia.
+
+      destruct (lookup_lt_is_Some_2 us 0) as (w_ & Hus_lookup); first lia.
+      iDestruct (array_cslice_update with "Hdata_cslice₂") as "(Hdata_back₂ & Hdata_cslice₂)"; first done.
+      iEval (rewrite Nat.add_0_r) in "Hdata_back₂ Hdata_cslice₂".
+
+      iDestruct (array_cslice_combine with "Hdata_back₁ Hdata_back₂") as "(%Heq & Hdata_back)"; first done. injection Heq as <-.
+      iEval (rewrite dfrac_op_own Qp.half_half) in "Hdata_back".
+
+      iAaccIntro with "[$Hdata_back]". 1: iSteps.
+
+      - iIntros "(_ & (Hdata_back₁ & Hdata_back₂)) !>".
+
+        iDestruct (array_cslice_app_1 with "Hdata_cslice₁_1 (Hdata_cslice₁_2 Hdata_back₁)") as "Hdata_cslice₁"; first done.
+        iEval (rewrite list_insert_id //) in "Hdata_cslice₁".
+
+        iDestruct ("Hdata_cslice₂" with "Hdata_back₂") as "Hdata_cslice₂".
+        iEval (rewrite list_insert_id //) in "Hdata_cslice₂".
+
+        iFrameSteps.
+
+      - iIntros "(Hdata_back₁ & Hdata_back₂) !>".
+
+        iDestruct (array_cslice_app_1 with "Hdata_cslice₁_1 (Hdata_cslice₁_2 Hdata_back₁)") as "Hdata_cslice₁"; first done.
+
+        iDestruct ("Hdata_cslice₂" with "Hdata_back₂") as "Hdata_cslice₂".
+
+        iSplitR "Howner₁ Ht_front_cache Hdata_cslice₂".
+        { iFrameSteps.
+          - iPureIntro. simpl_length.
+          - iExists state1.
+            destruct Hstate1 as [-> | ->]; iFrameSteps.
+        }
+        iIntros "H£ HΦ".
+
+        iMod (lc_fupd_elim_later with "H£ HΦ") as "HΦ".
+        iSteps. iPureIntro. simpl_length.
+    Qed.
+
+    #[local] Lemma resolve_spec_loser_1 t γ front1 front2 id :
+      front1 < front2 →
+      {{{
+        inv' t γ ∗
+        front_lb γ front2
+      }}}
+        Resolve (CAS (#t).[front]%V #front1 #(front1 + 1)) #γ.(ws_bdeque_1_name_prophet) (#front1, #id)%V
+      {{{
+        RET false;
+        True
+      }}}.
+    Proof.
+      iIntros "%Hloser %Φ ((:inv') & #Hfront_lb) HΦ".
+
+      iInv "Hinv" as "(:inv_inner =3)".
+      iDestruct (front_lb_valid with "Hfront_auth Hfront_lb") as %?.
+      wp_apply (prophet_multi_wp_resolve' with "Hprophet_model"); [done.. |].
+      wp_cas as Hcas; zoo_simplify in Hcas; last lia.
+      iIntros "!> %prophs %Hprophss3 Hprophet_model".
+      iSplitR "HΦ".
+      { iFrameSteps.
+        - iPureIntro => *.
+          rewrite fn_lookup_alter_ne; first lia.
+          auto.
+        - rewrite fn_lookup_insert_ne //. iSteps.
+      }
+      iSteps.
+    Qed.
+    #[local] Lemma resolve_spec_loser_2 t γ front id prophs0 :
+      head prophs0 ≠ Some id →
+      {{{
+        inv' t γ ∗
+        front_lb γ front ∗
+        prophet_multi_full prophet_identifier γ.(ws_bdeque_1_name_prophet_name) front prophs0
+      }}}
+        Resolve (CAS (#t).[front]%V #front #(front + 1)) #γ.(ws_bdeque_1_name_prophet) (#front, #id)%V
+      {{{
+        RET false;
+        front_lb γ (S front)
+      }}}.
+    Proof.
+      iIntros "%Hloser %Φ ((:inv') & #Hfront_lb & #Hprophet_full) HΦ".
+
+      iInv "Hinv" as "(:inv_inner =1)".
+      iDestruct (front_lb_valid with "Hfront_auth Hfront_lb") as %?.
+      wp_apply (prophet_multi_wp_resolve' with "Hprophet_model"); [done.. |].
+      wp_apply (wp_cas_nobranch' with "Ht_front") as (b) "%Hcas Ht_front".
+      iIntros "%prophs %Hprophss1 Hprophet_model".
+      destruct b; zoo_simplify in Hcas; first subst front1.
+
+      - iDestruct (prophet_multi_full_valid with "Hprophet_model Hprophet_full") as %->.
+        rewrite fn_lookup_alter Hpasts1 // in Hloser.
+
+      - iDestruct (front_lb_get with "Hfront_auth") as "#-#Hfront_lb_1".
+        iDestruct (front_lb_le (S front) with "Hfront_lb_1") as "-##Hfront_lb_1"; first lia.
+        iSplitR "HΦ".
+        { iFrameSteps.
+          - iPureIntro => *.
+            rewrite fn_lookup_alter_ne; first lia.
+            auto.
+          - rewrite fn_lookup_insert_ne //. iSteps.
+        }
+        iSteps.
+    Qed.
+    #[local] Lemma resolve_spec_winner_pop t γ front P id :
+      {{{
+        inv' t γ ∗
+        winner_pop γ front P
+      }}}
+        Resolve (CAS (#t).[front]%V #front #(front + 1)) #γ.(ws_bdeque_1_name_prophet) (#front, #id)%V
+      {{{
+        RET true;
+        ▷ P
+      }}}.
+    Proof.
+      iIntros "%Φ ((:inv') & Hwinner_pop) HΦ".
+
+      iInv "Hinv" as "(:inv_inner =1)".
+      wp_apply (prophet_multi_wp_resolve' with "Hprophet_model"); [done.. |].
+      wp_apply (wp_cas_nobranch' with "Ht_front") as (b) "%Hcas Ht_front".
+      iIntros "%prophs %Hprophss1 Hprophet_model".
+      iDestruct (inv_state_winner_pop with "Hstate Hwinner_pop") as "(%P_ & -> & #Heq & Hstate & Hwinner_pop)".
+      rewrite Hprophss1.
+      destruct b; zoo_simplify in Hcas; last congruence.
+      iMod (front_update with "Hfront_auth") as "Hfront_auth".
+      iDestruct "Hstate" as "[(:inv_state_nonempty_steal =1) | (:inv_state_emptyish_steal =1)]".
+
+      - iDestruct "Hwinner" as "(:winner_pending_1)".
+        destruct vs1 as [| v1 vs1] => /=; first naive_solver lia.
+
+        iMod "HP" as "(%vs & Hmodel₁ & _ & HP)".
+        iDestruct (model_agree with "Hmodel₁ Hmodel₂") as %->.
+        iMod (model_steal with "Hmodel₁ Hmodel₂") as "(Hmodel₁ & Hmodel₂) /=".
+        iMod ("HP" with "[$Hmodel₁ $Hhistory_at_front1 //]") as "HP".
+
+        iDestruct (array_cslice_rotation_right_1' (S front) 1 with "Hdata_cslice₁") as "Hdata_cslice₁"; [simpl_length/=; lia.. |].
+        eassert (rotation _ _ = vs1 ++ priv1 ++ [v1]) as ->.
+        { destruct_decide (γ.(ws_bdeque_1_name_capacity) = 1) as Heq | ?.
+          - rewrite -> Heq in *.
+            simpl in Hdata1.
+            assert (length vs1 = 0) as ->%nil_length_inv by lia.
+            assert (length priv1 = 0) as ->%nil_length_inv by lia.
+            done.
+          - rewrite Nat.mod_1_l; first lia.
+            rewrite rotation_S; first lia.
+            rewrite rotation_0 assoc //.
+        }
+
+        iSplitR "HP HΦ".
+        { destruct_decide (S front = back1) as <- | ?.
+
+          - simpl in Hvs1.
+            iExists Empty. iFrameSteps; iPureIntro.
+            + simpl_length/=. lia.
+            + intros.
+              rewrite fn_lookup_alter_ne; first lia.
+              apply Hpasts1; first lia.
+
+          - destruct vs1 as [| v2 vs1] => /=; first naive_solver lia.
+            simpl in Hvs1.
+            iMod (history_update _ v2 with "Hhistory_auth") as "(Hhistory_auth & #Hhistory_at)"; first done.
+            iExists Nonempty. iFrameSteps; iPureIntro.
+            + simpl_length/=. lia.
+            + intros.
+              rewrite fn_lookup_alter_ne; first lia.
+              apply Hpasts1; first lia.
+            + simpl_length/=. lia.
+        }
+        iIntros "!> {%}".
+
+        iApply "HΦ". iModIntro.
+        iRewrite "Heq" => //.
+
+      - assert (length vs1 = 0) as ->%nil_length_inv by lia.
+
+        iDestruct (array_cslice_rotation_right_1' (S back1) 1 with "Hdata_cslice₁") as "Hdata_cslice₁"; [simpl_length; lia.. |].
+        iEval (rewrite /= -(app_nil_l (rotation _ _))) in "Hdata_cslice₁".
+
+        iSplitR "HP HΦ".
+        { iExists Superempty. iFrameSteps; iPureIntro.
+          - simpl_length.
+          - intros.
+            rewrite fn_lookup_alter_ne; first lia.
+            apply Hpasts1; first lia.
+        }
+        iIntros "!> {%}".
+
+        iApply "HΦ". iModIntro.
+        iRewrite "Heq" => //.
+    Qed.
+    #[local] Lemma resolve_spec_winner_steal t γ front P id :
+      {{{
+        inv' t γ ∗
+        winner_steal γ front P
+      }}}
+        Resolve (CAS (#t).[front]%V #front #(front + 1)) #γ.(ws_bdeque_1_name_prophet) (#front, #id)%V
+      {{{
+        RET true;
+        front_lb γ (S front)
+      }}}.
+    Proof.
+      iIntros "%Φ ((:inv') & Hwinner_steal) HΦ".
+
+      iInv "Hinv" as "(:inv_inner =1)".
+      wp_apply (prophet_multi_wp_resolve' with "Hprophet_model"); [done.. |].
+      wp_apply (wp_cas_nobranch' with "Ht_front") as (b) "%Hcas Ht_front".
+      iIntros "%prophs %Hprophss1 Hprophet_model".
+      iDestruct (inv_state_winner_steal with "Hstate Hwinner_steal") as "(%P_ & -> & _ & (:inv_state_emptyish_pop =1) & Hwinner_steal)".
+      destruct b; zoo_simplify in Hcas; last congruence.
+      iMod (front_update with "Hfront_auth") as "Hfront_auth".
+      iDestruct (front_lb_get with "Hfront_auth") as "#Hfront_lb".
+
+      assert (length vs1 = 0) as ->%nil_length_inv by lia.
+
+      iDestruct (array_cslice_rotation_right_1' (S back1) 1 with "Hdata_cslice₁") as "Hdata_cslice₁"; [simpl_length; lia.. |].
+      iEval (rewrite /= -(app_nil_l (rotation _ _))) in "Hdata_cslice₁".
+
+      iSplitR "HΦ".
+      { iExists Superempty. iFrameSteps; iPureIntro.
+        - simpl_length.
+        - intros.
+          rewrite fn_lookup_alter_ne; first lia.
+          apply Hpasts1; first lia.
+      }
+      iSteps.
+    Qed.
+    #[local] Lemma resolve_spec_Empty t γ back ws id :
+      {{{
+        inv' t γ ∗
+        owner₁ γ Stable back ws ∗
+        front_lb γ back
+      }}}
+        Resolve (CAS (#t).[front]%V #back #(back + 1)) #γ.(ws_bdeque_1_name_prophet) (#back, #id)%V
+      {{{
+        RET true;
+        owner₁ γ Unstable back ws ∗
+        front_lb γ (S back)
+      }}}.
+    Proof.
+      iIntros "%Φ ((:inv') & Howner₁ & #Hfront_lb) HΦ".
+
+      iInv "Hinv" as "(:inv_inner =1)".
+      wp_apply (prophet_multi_wp_resolve' with "Hprophet_model"); [done.. |].
+      wp_apply (wp_cas_nobranch' with "Ht_front") as (b) "%Hcas Ht_front".
+      iIntros "%prophs %Hprophss1 Hprophet_model".
+      iDestruct (owner_agree with "Howner₁ Howner₂") as %(<- & <-).
+      iDestruct (front_lb_valid with "Hfront_auth Hfront_lb") as %?.
+      iDestruct (inv_state_Stable with "Hstate") as "#([-> | ->] & _)"; first done.
+
+      - iDestruct "Hstate" as "(:inv_state_empty =1 lazy=)".
+        assert (length vs1 = 0) as ->%nil_length_inv by lia.
+        destruct b; zoo_simplify in Hcas; last lia.
+
+        iMod (front_update with "Hfront_auth") as "Hfront_auth".
+        iClear "Hfront_lb". iDestruct (front_lb_get with "Hfront_auth") as "#Hfront_lb".
+        iMod (history_update _ inhabitant with "Hhistory_auth") as "(Hhistory_auth & _)"; first done.
+        iMod (owner_update Unstable (length hist1) with "Howner₁ Howner₂") as "(Howner₁ & Howner₂)".
+
+        iDestruct (array_cslice_rotation_right_1' (S (length hist1)) 1 with "Hdata_cslice₁") as "Hdata_cslice₁"; [simpl_length; lia.. |].
+        iEval (rewrite -(app_nil_l (rotation _ _ ))) in "Hdata_cslice₁".
+
+        iSplitR "Howner₁ HΦ".
+        { iExists Superempty. iFrameSteps; iPureIntro.
+          - simpl_length.
+          - intros.
+            rewrite fn_lookup_alter_ne; first lia.
+            apply Hpasts1; first lia.
+          - simpl_length/=. lia.
+        }
+        rewrite Hhist1. iSteps.
+
+      - iDestruct "Hstate" as "(:inv_state_nonempty =1 lazy=)".
+        exfalso. lia.
+    Qed.
+
+    Lemma ws_bdeque_1_size_spec t γ ι cap ws :
+      <<<
+        ws_bdeque_1_inv t γ ι cap ∗
+        ws_bdeque_1_owner t γ ws
+      | ∀∀ vs,
+        ws_bdeque_1_model γ vs
+      >>>
+        ws_bdeque_1_size #t @ ↑ι
+      <<<
+        ⌜vs `suffix_of` ws⌝ ∗
+        ws_bdeque_1_model γ vs
+      | RET #(length vs);
+        ws_bdeque_1_owner t γ vs
+      >>>.
+    Proof.
+      iIntros "%Φ ((:inv) & (:owner)) HΦ".
+      iDestruct "Howner" as "(:owner_2)".
+
+      wp_rec.
+
+      wp_bind (_.{front})%E.
+      iInv "Hinv" as "(:inv_inner =1)".
+      wp_load.
+      iDestruct (owner_agree with "Howner₁ Howner₂") as %(<- & <-).
+      iDestruct (inv_state_Stable with "Hstate") as %(_ & Hback); first done.
+
+      iMod "HΦ" as "(%vs & (:model) & _ & HΦ)".
+      iDestruct (model_owner₁_agree with "Howner₁ Hmodel₁ Hmodel₂") as %(Hsuffix & <-).
+      iMod (owner₁_update with "Howner₁ Hmodel₁ Hmodel₂") as "(Howner₁ & Hmodel₁ & Hmodel₂)".
+      iMod ("HΦ" with "[$Hmodel₁ //]") as "HΦ".
+
+      iSplitR "Howner₁ Ht_front_cache Hdata_cslice₂ HΦ". { iFrameSteps. }
+      iIntros "!> {%- Hcapacity Hfront_cache Hus Hvs1 Hback}".
+
+      wp_apply (back_spec with "[$Howner₁]") as "Howner₁"; first iSteps.
+      wp_pures.
+
+      replace (⁺back - ⁺front1)%Z with ⁺(length vs) by lia.
+      iSteps.
+    Qed.
+
+    Lemma ws_bdeque_1_is_empty_spec t γ ι cap ws :
+      <<<
+        ws_bdeque_1_inv t γ ι cap ∗
+        ws_bdeque_1_owner t γ ws
+      | ∀∀ vs,
+        ws_bdeque_1_model γ vs
+      >>>
+        ws_bdeque_1_is_empty #t @ ↑ι
+      <<<
+        ⌜vs `suffix_of` ws⌝ ∗
+        ws_bdeque_1_model γ vs
+      | RET #(bool_decide (vs = []%list));
+        ws_bdeque_1_owner t γ vs
+      >>>.
+    Proof.
+      iIntros "%Φ (#Hinv & Howner) HΦ".
+
+      wp_rec.
+      wp_apply (ws_bdeque_1_size_spec with "[$]").
+      iApply (atomic_update_wand with "HΦ"). iIntros "%vs HΦ (%Hvs & Howner)".
+      wp_pures.
+
+      rewrite (bool_decide_ext (⁺(length vs) = 0) (vs = [])).
+      { rewrite -length_zero_iff_nil. lia. }
+      iApply "HΦ".
+      iFrameSteps.
+    Qed.
+
+    #[local] Definition push_au t γ ws v Φ : iProp Σ :=
+      AU <{
+        ∃∃ vs,
+        ws_bdeque_1_model γ vs
+      }> @ ⊤ ∖ ↑γ.(ws_bdeque_1_name_inv), ∅ <{
+        ∀∀ b,
+        ⌜b = bool_decide (length vs < γ.(ws_bdeque_1_name_capacity))⌝ ∗
+        ⌜vs `suffix_of` ws⌝ ∗
+        ws_bdeque_1_model γ (if b then vs ++ [v] else vs)
+      , COMM
+        ws_bdeque_1_owner t γ (if b then vs ++ [v] else ws) -∗
+        Φ #b
+      }>.
+    Lemma ws_bdeque_1_push_spec t γ ι cap ws v :
+      <<<
+        ws_bdeque_1_inv t γ ι cap ∗
+        ws_bdeque_1_owner t γ ws
+      | ∀∀ vs,
+        ws_bdeque_1_model γ vs
+      >>>
+        ws_bdeque_1_push #t v @ ↑ι
+      <<<
+        ∃∃ b,
+        ⌜b = bool_decide (length vs < cap)⌝ ∗
+        ⌜vs `suffix_of` ws⌝ ∗
+        ws_bdeque_1_model γ (if b then vs ++ [v] else vs)
+      | RET #b;
+        ws_bdeque_1_owner t γ (if b then vs ++ [v] else ws)
+      >>>.
+    Proof.
+      iIntros "%Φ ((:inv) & (:owner)) HΦ".
+      rename us into us0. iDestruct (owner_2_rebase back with "Howner") as "(%us & (:owner_2))"; first done.
+
+      wp_rec.
+      wp_smart_apply (back_spec with "[$Howner₁]") as "Howner₁"; first iSteps.
+      wp_load.
+      wp_smart_apply (array_size_spec_cslice with "Hdata_cslice₂") as "Hdata_cslice₂".
+      wp_load. wp_pures.
+
+      wp_bind (_ or _)%E.
+      wp_apply (wp_wand (λ res,
+        ∃ b front_cache,
+        ⌜res = #b⌝ ∗
+        t.[front_cache] ↦ #front_cache ∗
+        front_lb γ front_cache ∗
+        owner₁ γ Stable back ws ∗
+        if b then
+          ⌜back < front_cache + γ.(ws_bdeque_1_name_capacity)⌝ ∗
+          push_au t γ ws v Φ
+        else
+          ⌜back ≤ front_cache + γ.(ws_bdeque_1_name_capacity)⌝ ∗
+          (ws_bdeque_1_owner t γ ws -∗ Φ false%V)
+      )%I with "[Howner₁ Ht_front_cache HΦ]") as (res) "{Hfront_lb_cache} {% front_cache Hfront_cache} (%b & %front_cache & -> & Ht_front_cache & #Hfront_lb_cache & Howner₁ & HΦ)".
+      { case_bool_decide; wp_pures.
+
+        - iStep. iFrame "#∗". iSteps.
+
+        - wp_rec.
+
+          wp_bind (_.{front})%E.
+          wp_apply (wp_wand (λ res,
+            ∃ front,
+            ⌜res = #front⌝ ∗
+            front_lb γ front ∗
+            owner₁ γ Stable back ws ∗
+            if bool_decide (front_cache < front) then
+              ⌜back < front + γ.(ws_bdeque_1_name_capacity)⌝ ∗
+              push_au t γ ws v Φ
+            else
+              ⌜back ≤ front + γ.(ws_bdeque_1_name_capacity)⌝ ∗
+              (ws_bdeque_1_owner t γ ws -∗ Φ false%V)
+          )%I with "[Howner₁ HΦ]") as (res) "(%front & -> & #Hfront_lb & Howner₁ & HΦ)".
+          { iInv "Hinv" as "(:inv_inner =1)".
+            wp_load.
+            iDestruct (owner_agree with "Howner₁ Howner₂") as %(<- & <-).
+            iDestruct (front_lb_get with "Hfront_auth") as "#$".
+            case_bool_decide. 1: iFrameSteps.
+
+            iMod "HΦ" as "(%vs & (:model) & _ & HΦ)".
+            iDestruct (model_owner₁_agree with "Howner₁ Hmodel₁ Hmodel₂") as %(Hsuffix & <-).
+            rewrite bool_decide_eq_false_2; first lia.
+            iMod ("HΦ" with "[Hmodel₁]") as "HΦ"; first iFrameSteps.
+
+            iFrameSteps.
+          }
+
+          wp_store. wp_pures.
+
+          iFrame "#∗". iPureIntro.
+          erewrite bool_decide_ext; [done | lia].
+      }
+
+      destruct b; wp_pures.
+
+      - iDestruct "HΦ" as "(%Hfront_cache & HΦ)".
+
+        wp_apply (array_unsafe_cset_spec_owner with "[$Howner₁ $Ht_front_cache $Hdata_cslice₂]") as "(:owner_2 !=)"; [done | iSteps |].
+        wp_pures.
+
+        wp_bind (_ <-{back} _)%E.
+        iInv "Hinv" as "(:inv_inner =2)".
+        wp_store.
+        iDestruct (owner_agree with "Howner₁ Howner₂") as %(<- & <-).
+        iMod (owner_update Stable (S back) with "Howner₁ Howner₂") as "(Howner₁ & Howner₂)".
+        iDestruct (inv_state_Stable with "Hstate") as "(%Hstate2 & %)"; first done.
+        iDestruct (front_lb_valid with "Hfront_auth Hfront_lb_cache") as %?.
+
+        iAssert ⌜head priv2 = Some v⌝%I as %(priv2' & ->)%head_Some.
+        { iDestruct (array_cslice_rotation_right_small_1' back (length vs2) with "Hdata_cslice₁") as "Hdata_cslice₁"; [simpl_length; lia.. |].
+          rewrite /rotation drop_app_length.
+          rewrite head_lookup -(lookup_app_l _ (take (length vs2) (vs2 ++ priv2))); first lia.
+          iDestruct (array_cslice_agree with "Hdata_cslice₁ Hdata_cslice₂") as %->.
+          { simpl_length. lia. }
+          rewrite list_lookup_insert_eq //; first lia.
+        }
+        iEval (rewrite (assoc _ _ [_])) in "Hdata_cslice₁".
+
+        iMod "HΦ" as "(%vs & (:model) & _ & HΦ)".
+        iDestruct (model_owner₁_agree with "Howner₁ Hmodel₁ Hmodel₂") as %(Hsuffix & <-).
+        iMod (model_push v with "Howner₁ Hmodel₁ Hmodel₂") as "(Howner₁ & Hmodel₁ & Hmodel₂)".
+        iMod ("HΦ" $! true with "[$Hmodel₁]") as "HΦ".
+        { iSteps; iPureIntro.
+          - rewrite bool_decide_eq_true_2 //; first lia.
+          - simpl_length/=. lia.
+        }
+
+        iSplitR "Howner₁ Ht_front_cache Hdata_cslice₂ HΦ".
+        { iExists Nonempty.
+          destruct Hstate2 as [-> | ->].
+
+          - iDestruct "Hstate" as "(:inv_state_empty =1 lazy=)".
+            assert (length vs = 0) as ->%nil_length_inv by lia.
+            iMod (history_update back v with "Hhistory_auth") as "(Hhistory_auth & #Hhistory_at)"; first done.
+            iFrameSteps. iPureIntro.
+            simpl_length/=. lia.
+
+          - iDestruct "Hstate" as "(:inv_state_nonempty =1 lazy=)".
+            iFrameSteps; try iPureIntro.
+            + simpl_length/=. lia.
+            + simpl_length/=. lia.
+            + rewrite hd_app //; first lia.
+        }
+        iIntros "!> {%- Hcapacity Hfront_cache Hus}".
+
+        iSteps. iPureIntro. simpl_length.
+
+      - iDestruct "HΦ" as "(%Hfront_cache & HΦ)".
+
+        iApply "HΦ".
+        iFrameSteps.
+    Qed.
+
+    Lemma ws_bdeque_1_steal_spec t γ ι cap :
+      <<<
+        ws_bdeque_1_inv t γ ι cap
+      | ∀∀ vs,
+        ws_bdeque_1_model γ vs
+      >>>
+        ws_bdeque_1_steal #t @ ↑ι
+      <<<
+        ws_bdeque_1_model γ (tail vs)
+      | RET head vs;
+        True
+      >>>.
+    Proof.
+      iIntros "%Φ (:inv) HΦ".
+
+      iLöb as "HLöb".
+
+      wp_rec.
+      wp_apply (wp_id with "[//]") as (id) "Hid".
+      wp_smart_apply front_spec as (front1) "#Hfront_lb_1"; first iSteps.
+      wp_pures.
+
+      wp_bind (_.{back})%E.
+      iInv "Hinv" as "(:inv_inner =2)".
+      wp_load.
+      iDestruct (front_lb_valid with "Hfront_auth Hfront_lb_1") as %?.
+
+      destruct_decide (front1 < back2) as Hbranch1; last first.
+      { assert (length vs2 = 0) as ->%nil_length_inv by lia.
+
+        iMod "HΦ" as "(%vs & (:model) & _ & HΦ)".
+        iDestruct (model_agree with "Hmodel₁ Hmodel₂") as %->.
+        iMod ("HΦ" with "[$Hmodel₁ //] [//]") as "HΦ".
+
+        iFrameSteps.
+      }
+
+      destruct_decide (front1 = front2) as <- | ?; last first.
+      { assert (front1 < front2) as Hbranch2 by lia.
+        iDestruct (front_lb_get with "Hfront_auth") as "#Hfront_lb_2".
+        iSplitR "HΦ". { iFrameSteps. }
+        iIntros "!> {%- Hcapacity Hbranch1 Hbranch2}".
+
+        wp_pures.
+        rewrite bool_decide_eq_false_2; first lia.
+        wp_load.
+        wp_smart_apply array_unsafe_cget_spec_loser as (v) "_"; [lia | iSteps |].
+        wp_load.
+        wp_smart_apply resolve_spec_loser_1; [done | iSteps |].
+        iSteps.
+      }
+
+      iDestruct (prophet_multi_full_get _ front1 with "Hprophet_model") as "#Hprophet_full".
+      iEval (rewrite Hpasts2 //=) in "Hprophet_full".
+
+      destruct_decide (head $ prophss2 front1 = Some id) as (prophs0 & Hbranch3)%head_Some | Hbranch3; last first.
+      { iSplitR "HΦ". { iFrameSteps. }
+        remember (prophss2 front1) as prophs0.
+        iIntros "!> {%- Hcapacity Hbranch1 Hbranch3}".
+
+        wp_pures.
+        rewrite bool_decide_eq_false_2; first lia.
+        wp_load.
+        wp_smart_apply array_unsafe_cget_spec_loser as (v) "_"; [lia | iSteps |].
+        wp_load.
+        wp_smart_apply resolve_spec_loser_2; [done | iSteps |].
+        iSteps.
+      }
+      rewrite Hbranch3.
+
+      iDestruct (inv_state_Nonempty with "Hstate") as %->; first done.
+      iDestruct "Hstate" as "(:inv_state_nonempty =2)".
+      iDestruct "Hwinner" as "[(:winner) | (:winner_pending_2 !=)]"; last first.
+      { iDestruct (identifier_model_exclusive with "Hid Hid_") as %[]. }
+
+      destruct vs2 as [| v vs2] => /=; first naive_solver lia.
+      iMod (winner_update front1 (Φ (Some v)) with "Hwinner_pop Hwinner_steal") as "(Hwinner_pop & Hwinner_steal)".
+
+      iSplitR "Hwinner_pop".
+      { iExists Nonempty. iFrameSteps.
+        rewrite Hbranch3 /winner_pending_2. iSteps. iIntros "!> !>".
+        rewrite /winner_au. iAuIntro.
+        iApply (aacc_aupd_commit with "HΦ"); first done. iIntros "%vs (:model)".
+        iAaccIntro with "Hmodel₁"; first iSteps. iIntros "%v_ %vs' (-> & Hmodel₁ & Hhistory_at) !>".
+        iDestruct (history_at_agree with "Hhistory_at Hhistory_at_front2") as %<-.
+        simpl in Hvs. iSteps.
+      }
+      iIntros "!> {%- Hcapacity Hbranch1}".
+
+      wp_pures.
+      rewrite bool_decide_eq_false_2; first lia.
+      wp_load.
+      wp_smart_apply (array_unsafe_cget_spec_winner_pop with "[$Hwinner_pop]") as "Hwinner_pop"; first iSteps.
+      wp_load.
+      wp_smart_apply (resolve_spec_winner_pop with "[$Hwinner_pop]") as "HΦ"; first iSteps.
+      iSteps.
+    Qed.
+
+    Inductive pop_state :=
+      | PopNonempty v
+      | PopEmptyishWinner v
+      | PopEmptyishLoser
+      | PopSuperempty.
+    #[local] Lemma ws_bdeque_1_pop_0_spec {t γ} (state : pop_state) {stable} back ws front_cache us id (back_ : Z) :
+      back_ = back →
+      {{{
+        inv' t γ ∗
+        owner_1 OwnerPop t γ stable back ws front_cache back us ∗
+        match state with
+        | PopNonempty v =>
+            ⌜stable = Stable⌝ ∗
+            ⌜us !! 0 = Some v⌝
+        | PopEmptyishWinner v =>
+            ⌜stable = Unstable⌝ ∗
+            ⌜us !! 0 = Some v⌝ ∗
+            winner_steal γ back inhabitant
+        | PopEmptyishLoser =>
+            ∃ id_winner prophs,
+            ⌜stable = Unstable⌝ ∗
+            prophet_multi_full prophet_identifier γ.(ws_bdeque_1_name_prophet_name) back (id_winner :: prophs) ∗
+            ⌜head (id_winner :: prophs) ≠ Some id⌝
+        | PopSuperempty =>
+            ∃ front,
+            ⌜stable = Unstable⌝ ∗
+            front_lb γ front ∗
+            ⌜front = S back⌝
+        end
+      }}}
+        ws_bdeque_1_pop_0 #t #id #back_
+      {{{ o back front_cache i us,
+        RET o;
+        owner_2 t γ Stable back ws front_cache i us ∗
+        match state with
+        | PopNonempty v =>
+            ⌜o = Some v⌝
+        | PopEmptyishWinner v =>
+            ⌜o = Some v⌝
+        | PopEmptyishLoser =>
+            ⌜o = None⌝
+        | PopSuperempty =>
+            ⌜o = None⌝
+        end
+      }}}.
+    Proof.
+      iIntros (->) "%Φ ((:inv') & (:owner_1) & H) HΦ".
+
+      wp_rec. wp_pures.
+      destruct state.
+
+      - iDestruct "H" as "(-> & %Hus_lookup)".
+        iSpecialize ("HΦ" $! (Some v)).
+
+        wp_apply (front_spec_owner_Stable with "[$Howner₁]") as (front2) "(Howner₁ & #Hfront_lb & %Hfront2)"; first iSteps.
+        wp_pures.
+        rewrite bool_decide_eq_false_2; first lia.
+        wp_pures.
+        case_bool_decide as Hbranch; wp_pures.
+
+        + wp_load.
+          wp_apply (array_unsafe_cget_spec with "Hdata_cslice₂"); [done.. | lia |].
+          iSteps.
+
+        + replace front2 with back by lia.
+
+          wp_store. wp_load.
+          wp_smart_apply (resolve_spec_Empty with "[$Howner₁]") as "{Hfront_lb} (Howner₁ & #Hfront_lb)"; first iSteps.
+          wp_smart_apply (set_back_spec_Superempty with "[$Howner₁ $Hfront_lb]") as "Howner₁"; [lia.. | iSteps |].
+          wp_load.
+          wp_apply (array_unsafe_cget_spec with "Hdata_cslice₂") as "Hdata_cslice₂"; [done.. | lia |].
+          wp_pures.
+
+          iApply "HΦ".
+          iFrame "#∗". iSteps.
+
+      - iDestruct "H" as "(-> & %Hus_lookup & Hwinner_steal)".
+        iSpecialize ("HΦ" $! (Some v)).
+
+        wp_apply (front_spec_winner_steal with "[$Hwinner_steal]") as "Hwinner_steal"; first iSteps.
+        wp_pures.
+        rewrite bool_decide_eq_false_2; first lia.
+        wp_pures.
+        rewrite bool_decide_eq_false_2; first lia.
+        wp_store. wp_load.
+        wp_smart_apply (resolve_spec_winner_steal with "[$Hwinner_steal]") as "#Hfront_lb"; first iSteps.
+        wp_smart_apply (set_back_spec_Superempty with "[$Howner₁ $Hfront_lb]") as "Howner₁"; [lia.. | iSteps |].
+        wp_load.
+        wp_apply (array_unsafe_cget_spec with "Hdata_cslice₂") as "Hdata_cslice₂"; [done.. | lia |].
+        wp_pures.
+
+        iApply "HΦ".
+        iFrame "#∗". iSteps.
+
+      - iDestruct "H" as "(%id_winner & %prophs & -> & #Hprophet_full & %Hloser)".
+        iSpecialize ("HΦ" $! None).
+
+        wp_apply (front_spec_owner_Unstable with "[$Howner₁]") as (front2) "(Howner₁ & #Hfront_lb & %Hbranch)"; first iSteps.
+        wp_pures.
+        destruct Hbranch as [-> | ->].
+
+        + rewrite bool_decide_eq_false_2; first lia.
+          wp_pures.
+          rewrite bool_decide_eq_false_2; first lia.
+          wp_store. wp_load.
+          wp_smart_apply (resolve_spec_loser_2 with "[$Hfront_lb $Hprophet_full]") as "{Hfront_lb} #Hfront_lb"; [done | iSteps |].
+          wp_smart_apply (set_back_spec_Superempty with "[$Howner₁ $Hfront_lb]") as "Howner₁"; [lia.. | iSteps |].
+          wp_pures.
+
+          iApply "HΦ".
+          iFrame "#∗". iSteps.
+
+        + rewrite bool_decide_eq_true_2; first lia.
+          wp_smart_apply (set_back_spec_Superempty with "[$Howner₁ $Hfront_lb]") as "Howner₁"; [lia.. | iSteps |].
+          iSteps.
+
+      - iDestruct "H" as "(%front & -> & #Hfront_lb & ->)".
+        iSpecialize ("HΦ" $! None).
+
+        wp_apply (front_spec_Superempty with "[$Howner₁ $Hfront_lb]") as "Howner₁"; [lia | iSteps |].
+        wp_pures.
+        rewrite bool_decide_eq_true_2; first lia.
+        wp_smart_apply (set_back_spec_Superempty with "[$Howner₁ $Hfront_lb]") as "Howner₁"; [lia.. | iSteps |].
+        iSteps.
+    Qed.
+    Lemma ws_bdeque_1_pop_spec t γ ι cap ws :
+      <<<
+        ws_bdeque_1_inv t γ ι cap ∗
+        ws_bdeque_1_owner t γ ws
+      | ∀∀ vs,
+        ws_bdeque_1_model γ vs
+      >>>
+        ws_bdeque_1_pop #t @ ↑ι
+      <<<
+        ∃∃ o ws',
+        ⌜vs `suffix_of` ws⌝ ∗
+        match o with
+        | None =>
+            ⌜vs = []⌝ ∗
+            ⌜ws' = []⌝ ∗
+            ws_bdeque_1_model γ []
+        | Some v =>
+            ∃ vs',
+            ⌜vs = vs' ++ [v]⌝ ∗
+            ⌜ws' = vs'⌝ ∗
+            ws_bdeque_1_model γ vs'
+        end
+      | RET o;
+        ws_bdeque_1_owner t γ ws'
+      >>>.
+    Proof.
+      iIntros "%Φ ((:inv) & (:owner)) HΦ".
+      rename us into us0. iDestruct (owner_2_rebase (back - 1) with "Howner") as "(%us & (:owner_2))"; first done.
+
+      wp_rec.
+      wp_apply (wp_id with "[//]") as (id) "Hid".
+      wp_smart_apply (back_spec with "[$Howner₁]") as "Howner₁"; first iSteps.
+      wp_pures.
+
+      wp_bind (_ <-{back} _)%E.
+      iInv "Hinv" as "(:inv_inner =1)".
+      wp_store.
+      iDestruct (owner_agree with "Howner₁ Howner₂") as %(<- & <-).
+      iDestruct (inv_state_Stable with "Hstate") as "#(%Hstate1 & %)"; first done.
+      destruct Hstate1 as [-> | ->].
+
+      { iDestruct "Hstate" as "(:inv_state_empty =1 lazy=)".
+        assert (0 < back) as Hback by lia.
+        assert (length vs1 = 0) as ->%nil_length_inv by lia.
+
+        iDestruct (front_lb_get with "Hfront_auth") as "#Hfront_lb".
+        iMod (owner_update Unstable (back - 1) with "Howner₁ Howner₂") as "(Howner₁ & Howner₂)".
+
+        iMod "HΦ" as "(%vs & (:model) & _ & HΦ)".
+        iDestruct (model_owner₁_agree with "Howner₁ Hmodel₁ Hmodel₂") as %(Hsuffix & ->).
+        iMod (model_empty with "Howner₁ Hmodel₁ Hmodel₂") as "(Howner₁ & Hmodel₁ & Hmodel₂)".
+        iMod ("HΦ" $! None with "[$Hmodel₁ //]") as "HΦ".
+
+        iSplitR "Howner₁ Ht_front_cache Hdata_cslice₂ HΦ".
+        { iExists Superempty. iFrameSteps. }
+        iIntros "!> {%- Hcapacity Hfront_cache Hus Hback}".
+
+        wp_smart_apply (ws_bdeque_1_pop_0_spec PopSuperempty (back - 1) with "[- HΦ]"); [lia | iFrameSteps |].
+        iSteps.
+      }
+
+      iDestruct "Hstate" as "(:inv_state_nonempty =1 lazy=)".
+      assert (0 < back) as Hback by lia.
+      destruct vs1 as [| v vs1 _] using rev_ind; first naive_solver lia.
+      simpl_length/= in Hvs1.
+      simpl_length/= in Hdata1.
+
+      destruct_decide (S front1 = back) as <- | Hbranch1.
+
+      - assert (length vs1 = 0) as ->%nil_length_inv.
+        { simpl_length/= in Hvs1. lia. }
+        simpl in *.
+        iEval (rewrite Nat.sub_0_r) in "Hdata_cslice₂".
+
+        iAssert ⌜us !! 0 = Some v⌝%I as %Hus_lookup.
+        { iDestruct (array_cslice_agree with "Hdata_cslice₁ Hdata_cslice₂") as %<-; first (simpl; lia).
+          iSteps.
+        }
+
+        iMod (owner_update Unstable front1 with "Howner₁ Howner₂") as "(Howner₁ & Howner₂)".
+
+        destruct_decide (head $ prophss1 front1 = Some id) as (prophs0 & Hprophss1)%head_Some | Hbranch2.
+
+        + rewrite Hprophss1.
+          iDestruct "Hwinner" as "[(:winner) | (:winner_pending_2 !=)]"; last first.
+          { iDestruct (identifier_model_exclusive with "Hid Hid_") as %[]. }
+          iMod (winner_update front1 inhabitant with "Hwinner_pop Hwinner_steal") as "(Hwinner_pop & Hwinner_steal)".
+
+          iMod "HΦ" as "(%vs & (:model) & _ & HΦ)".
+          iDestruct (model_owner₁_agree with "Howner₁ Hmodel₁ Hmodel₂") as %(Hsuffix & ->).
+          iMod (model_pop with "Howner₁ Hmodel₁ Hmodel₂") as "(Howner₁ & Hmodel₁ & Hmodel₂) /=".
+          iMod ("HΦ" $! (Some v) with "[$Hmodel₁]") as "HΦ"; first iSteps.
+
+          iSplitR "Howner₁ Ht_front_cache Hdata_cslice₂ Hwinner_steal HΦ".
+          { iExists Emptyish. iFrameSteps. }
+          iIntros "!> {%- Hcapacity Hfront_cache Hus Hback Hus_lookup}".
+
+          wp_smart_apply (ws_bdeque_1_pop_0_spec (PopEmptyishWinner v) front1 with "[- HΦ]"); [lia | iFrameSteps |].
+          iSteps.
+
+        + iDestruct "Hwinner" as "[(:winner) | Hwinner]".
+
+          { iMod (winner_update front1 inhabitant with "Hwinner_pop Hwinner_steal") as "(Hwinner_pop & Hwinner_steal)".
+
+            iMod "HΦ" as "(%vs & (:model) & _ & HΦ)".
+            iDestruct (model_owner₁_agree with "Howner₁ Hmodel₁ Hmodel₂") as %(Hsuffix & ->).
+            iMod (model_pop with "Howner₁ Hmodel₁ Hmodel₂") as "(Howner₁ & Hmodel₁ & Hmodel₂) /=".
+            iMod ("HΦ" $! (Some v) with "[$Hmodel₁]") as "HΦ"; first iSteps.
+
+            iSplitR "Howner₁ Ht_front_cache Hdata_cslice₂ Hwinner_steal HΦ".
+            { iExists Emptyish. iFrameSteps. }
+            iIntros "!> {%- Hcapacity Hfront_cache Hus Hus_lookup}".
+
+            wp_smart_apply (ws_bdeque_1_pop_0_spec (PopEmptyishWinner v) front1 with "[- HΦ]"); [lia | iFrameSteps |].
+            iSteps.
+          }
+
+          iDestruct (prophet_multi_full_get _ front1 with "Hprophet_model") as "#Hprophet_full".
+          iEval (rewrite Hpasts1 //=) in "Hprophet_full".
+          destruct (prophss1 front1) as [| id_winner prophs]; first done.
+          iDestruct "Hwinner" as "(:winner_pending_2 !=)".
+
+          iMod "HP" as "(%vs & Hmodel₁ & _ & HP)".
+          iDestruct (model_agree with "Hmodel₁ Hmodel₂") as %->.
+          iMod (model_steal with "Hmodel₁ Hmodel₂") as "(Hmodel₁ & Hmodel₂) /=".
+          iMod ("HP" with "[$Hmodel₁]") as "HP"; first iSteps.
+
+          iMod "HΦ" as "(%vs & (:model) & _ & HΦ)".
+          iDestruct (model_owner₁_agree with "Howner₁ Hmodel₁ Hmodel₂") as %(Hsuffix & ->).
+          iMod (model_empty with "Howner₁ Hmodel₁ Hmodel₂") as "(Howner₁ & Hmodel₁ & Hmodel₂)".
+          iMod ("HΦ" $! None with "[$Hmodel₁ //]") as "HΦ".
+
+          iSplitR "Howner₁ Ht_front_cache Hdata_cslice₂ HΦ".
+          { iExists Emptyish. iFrameStep 7. iExists P. iSteps. }
+          iIntros "!> {%- Hcapacity Hfront_cache Hus Hbranch2}".
+
+          wp_smart_apply (ws_bdeque_1_pop_0_spec PopEmptyishLoser front1 with "[- HΦ]"); [lia | iFrameSteps |].
+          iSteps.
+
+      - iMod (owner_update Stable (back - 1) with "Howner₁ Howner₂") as "(Howner₁ & Howner₂)".
+        iEval (rewrite -assoc) in "Hdata_cslice₁".
+
+        iMod "HΦ" as "(%vs & (:model) & _ & HΦ)".
+        iDestruct (model_owner₁_agree with "Howner₁ Hmodel₁ Hmodel₂") as %(Hsuffix & ->).
+        iMod (model_pop' with "Howner₁ Hmodel₁ Hmodel₂") as "(Howner₁ & Hmodel₁ & Hmodel₂)".
+        iMod ("HΦ" $! (Some v) with "[$Hmodel₁]") as "HΦ"; first iSteps.
+
+        iAssert ⌜us !! 0 = Some v⌝%I as %Hus_lookup.
+        { iDestruct (array_cslice_rotation_right_small_1' (back - 1) (length vs1) with "Hdata_cslice₁") as "Hdata_cslice₁"; [simpl_length/=; lia.. |].
+          iDestruct (array_cslice_agree with "Hdata_cslice₁ Hdata_cslice₂") as %<-.
+          { simpl_length/=. lia. }
+          rewrite /rotation drop_app_length //.
+        }
+
+        iSplitR "Howner₁ Ht_front_cache Hdata_cslice₂ HΦ".
+        { iExists Nonempty. iFrameSteps.
+          rewrite hd_app //; first lia.
+        }
+        iIntros "!> {%- Hcapacity Hfront_cache Hus Hback Hus_lookup}".
+
+        wp_smart_apply (ws_bdeque_1_pop_0_spec (PopNonempty v) (back - 1) with "[- HΦ]"); [lia | iFrameSteps |].
+        iSteps.
+    Qed.
+  End ws_bdeque_1_G.
+
+  #[global] Opaque ws_bdeque_1_inv.
+  #[global] Opaque ws_bdeque_1_model.
+  #[global] Opaque ws_bdeque_1_owner.
+End base.
+
+From zoo_saturn Require
+  ws_bdeque_1__opaque.
+
+Section ws_bdeque_1_G.
+  Context `{ws_bdeque_1_G : WsBdeque1G Σ}.
+
+  Implicit Types 𝑡 : location.
+  Implicit Types t : val.
+
   Definition ws_bdeque_1_inv t ι cap : iProp Σ :=
-    ∃ l γ,
-    ⌜t = #l⌝ ∗
-    ⌜ι = γ.(metadata_inv)⌝ ∗
-    ⌜cap = γ.(metadata_capacity)⌝ ∗
-    meta l nroot γ ∗
-    inv' l γ.
+    ∃ 𝑡 γ,
+    ⌜t = #𝑡⌝ ∗
+    meta 𝑡 nroot γ ∗
+    base.ws_bdeque_1_inv 𝑡 γ ι cap.
   #[local] Instance : CustomIpat "inv" :=
-    " ( %l &
-        %γ &
-        -> &
-        -> &
-        -> &
-        #Hmeta &
-        (:inv')
+    " ( %𝑡{} &
+        %γ{} &
+        {%Heq{};->} &
+        #Hmeta{_{}} &
+        Hinv{_{}}
       )
     ".
 
   Definition ws_bdeque_1_model t vs : iProp Σ :=
-    ∃ l γ,
-    ⌜t = #l⌝ ∗
-    meta l nroot γ ∗
-    model₁ γ vs ∗
-    ⌜length vs ≤ γ.(metadata_capacity)⌝.
+    ∃ 𝑡 γ,
+    ⌜t = #𝑡⌝ ∗
+    meta 𝑡 nroot γ ∗
+    base.ws_bdeque_1_model γ vs.
   #[local] Instance : CustomIpat "model" :=
-    " ( %l{;_} &
-        %γ{;_} &
-        %Heq{} &
-        Hmeta_{} &
-        Hmodel₁{_{}} &
-        %Hvs{}
+    " ( %𝑡{} &
+        %γ{} &
+        {%Heq{};->} &
+        #Hmeta{_{}} &
+        Hmodel{_{}}
       )
     ".
 
-  Inductive owner_flag :=
-    | OwnerNormal
-    | OwnerPop.
-  #[local] Definition owner_1 flag l γ stable back ws front_cache i us : iProp Σ :=
-    owner₁ γ stable back ws ∗
-    l.[front_cache] ↦ #front_cache ∗
-    front_lb γ front_cache ∗
-    ⌜(if flag is OwnerPop then S back else back) ≤ front_cache + γ.(metadata_capacity)⌝ ∗
-    array_cslice γ.(metadata_data) γ.(metadata_capacity) i (DfracOwn (1/2)) us ∗
-    ⌜length us = γ.(metadata_capacity)⌝.
-  #[local] Instance : CustomIpat "owner_1" :=
-    " ( Howner₁{_{}} &
-        Hl_front_cache{_{}} &
-        { {!} _
-        ; #Hfront_lb_cache_{}
-        ; #Hfront_lb_cache
-        } &
-        { {!} _
-        ; %Hfront_cache_{}
-        ; %Hfront_cache
-        } &
-        Hdata_cslice₂{_{}} &
-        { {!} _
-        ; %Hus{}
-        ; %Hus
-        }
-      )
-    ".
-  #[local] Definition owner_2 :=
-    owner_1 OwnerNormal.
-  #[local] Instance : CustomIpat "owner_2" :=
-    "(:owner_1)".
   Definition ws_bdeque_1_owner t ws : iProp Σ :=
-    ∃ l γ back front_cache i us,
-    ⌜t = #l⌝ ∗
-    meta l nroot γ ∗
-    owner_2 l γ Stable back ws front_cache i us.
+    ∃ 𝑡 γ,
+    ⌜t = #𝑡⌝ ∗
+    meta 𝑡 nroot γ ∗
+    base.ws_bdeque_1_owner 𝑡 γ ws.
   #[local] Instance : CustomIpat "owner" :=
-    " ( %l{;_} &
-        %γ{;_} &
-        %back{} &
-        %front_cache{_{}} &
-        %i{} &
-        %us{} &
-        %Heq{} &
-        Hmeta_{} &
+    " ( %𝑡{} &
+        %γ{} &
+        {%Heq{};->} &
+        #Hmeta{_{}} &
         Howner{_{}}
       )
     ".
 
-  #[global] Instance ws_bdeque_1_model_timeless t vs :
-    Timeless (ws_bdeque_1_model t vs).
+  #[global] Instance ws_bdeque_1_model_timeless γ vs :
+    Timeless (ws_bdeque_1_model γ vs).
   Proof.
     apply _.
   Qed.
-  #[global] Instance ws_bdeque_1_owner_timeless t ws :
-    Timeless (ws_bdeque_1_owner t ws).
+  #[global] Instance ws_bdeque_1_owner_timeless γ ws :
+    Timeless (ws_bdeque_1_owner γ ws).
   Proof.
     apply _.
   Qed.
@@ -517,294 +2219,14 @@ Section ws_bdeque_1_G.
     apply _.
   Qed.
 
-  #[local] Lemma model_owner_alloc :
-    ⊢ |==>
-      ∃ γ_model γ_owner,
-      model₁' γ_model [] ∗
-      model₂' γ_model [] ∗
-      owner₁' γ_owner γ_model Stable 1 [] ∗
-      owner₂' γ_owner Stable 1.
-  Proof.
-    iMod (auth_twins_alloc _ (auth_twins_G := ws_bdeque_1_G_model_G)) as "(%γ_model & Hmodel_auth & Hmodel₁ & Hmodel₂)".
-    iMod (twins_alloc' (twins_G := ws_bdeque_1_G_owner_G)) as "(%γ_owner & Howner₁ & Howner₂)".
-    iFrameSteps.
-  Qed.
-  #[local] Lemma model₁_valid γ stable back ws vs :
-    owner₁ γ stable back ws -∗
-    model₁ γ vs -∗
-    ⌜vs `suffix_of` ws⌝.
-  Proof.
-    iIntros "(:owner₁) Hmodel₁".
-    iDestruct (auth_twins_valid_1 with "Hmodel_auth Hmodel₁") as %H.
-    rewrite preorder_rtc in H. iSteps.
-  Qed.
-  #[local] Lemma model₁_exclusive γ vs1 vs2 :
-    model₁ γ vs1 -∗
-    model₁ γ vs2 -∗
-    False.
-  Proof.
-    apply auth_twins_twin1_exclusive.
-  Qed.
-  #[local] Lemma model_agree γ vs1 vs2 :
-    model₁ γ vs1 -∗
-    model₂ γ vs2 -∗
-    ⌜vs1 = vs2⌝.
-  Proof.
-    apply: auth_twins_agree_L.
-  Qed.
-  #[local] Lemma model_owner₁_agree γ stable back ws vs1 vs2 :
-    owner₁ γ stable back ws -∗
-    model₁ γ vs1 -∗
-    model₂ γ vs2 -∗
-      ⌜vs1 `suffix_of` ws⌝ ∗
-      ⌜vs1 = vs2⌝.
-  Proof.
-    iIntros "Howner₁ Hmodel₁ Hmodel₂".
-    iDestruct (model₁_valid with "Howner₁ Hmodel₁") as %Hsuffix.
-    iDestruct (model_agree with "Hmodel₁ Hmodel₂") as %->.
-    iSteps.
-  Qed.
-  #[local] Lemma model_empty {γ stable back ws vs1 vs2} :
-    owner₁ γ stable back ws -∗
-    model₁ γ vs1 -∗
-    model₂ γ vs2 ==∗
-      owner₁ γ stable back [] ∗
-      model₁ γ [] ∗
-      model₂ γ [].
-  Proof.
-    iIntros "(:owner₁) Hmodel₁ Hmodel₂".
-    iMod (auth_twins_update_auth with "Hmodel_auth Hmodel₁ Hmodel₂") as "(Hmodel_auth & Hmodel₁ & Hmodel₂)".
-    iSteps.
-  Qed.
-  #[local] Lemma model_push {γ stable back ws vs1 vs2} v :
-    owner₁ γ stable back ws -∗
-    model₁ γ vs1 -∗
-    model₂ γ vs2 ==∗
-      owner₁ γ stable back (vs1 ++ [v]) ∗
-      model₁ γ (vs1 ++ [v]) ∗
-      model₂ γ (vs1 ++ [v]).
-  Proof.
-    iIntros "(:owner₁) Hmodel₁ Hmodel₂".
-    iMod (auth_twins_update_auth with "Hmodel_auth Hmodel₁ Hmodel₂") as "(Hmodel_auth & Hmodel₁ & Hmodel₂)".
-    iSteps.
-  Qed.
-  #[local] Lemma model_steal γ vs1 vs2 :
-    model₁ γ vs1 -∗
-    model₂ γ vs2 ==∗
-      model₁ γ (tail vs1) ∗
-      model₂ γ (tail vs1).
-  Proof.
-    apply: auth_twins_update_twins_L.
-    rewrite preorder_rtc. apply suffix_tail. done.
-  Qed.
-  #[local] Lemma model_pop γ stable back ws vs1 vs2 :
-    owner₁ γ stable back ws -∗
-    model₁ γ vs1 -∗
-    model₂ γ vs2 ==∗
-      owner₁ γ stable back (removelast vs1) ∗
-      model₁ γ (removelast vs1) ∗
-      model₂ γ (removelast vs1).
-  Proof.
-    iIntros "(:owner₁) Hmodel₁ Hmodel₂".
-    iMod (auth_twins_update_auth with "Hmodel_auth Hmodel₁ Hmodel₂") as "(Hmodel_auth & Hmodel₁ & Hmodel₂)".
-    iSteps.
-  Qed.
-  #[local] Lemma model_pop' γ stable back ws vs1 v vs2 :
-    owner₁ γ stable back ws -∗
-    model₁ γ (vs1 ++ [v]) -∗
-    model₂ γ vs2 ==∗
-      owner₁ γ stable back vs1 ∗
-      model₁ γ vs1 ∗
-      model₂ γ vs1.
-  Proof.
-    rewrite -{2 3 4}(removelast_last vs1 v).
-    apply model_pop.
-  Qed.
-
-  #[local] Lemma owner₁_exclusive γ stable1 back1 ws1 stable2 back2 ws2 :
-    owner₁ γ stable1 back1 ws1 -∗
-    owner₁ γ stable2 back2 ws2 -∗
-    False.
-  Proof.
-    iIntros "(:owner₁ =1) (:owner₁ =2)".
-    iApply (twins_twin1_exclusive with "Howner₁_1 Howner₁_2").
-  Qed.
-  #[local] Lemma owner_agree γ stable1 back1 ws stable2 back2 :
-    owner₁ γ stable1 back1 ws -∗
-    owner₂ γ stable2 back2 -∗
-      ⌜stable1 = stable2⌝ ∗
-      ⌜back1 = back2⌝.
-  Proof.
-    iIntros "(:owner₁) Howner₂".
-    iDestruct (twins_agree_L with "Howner₁ Howner₂") as %[= <- <-].
-    iSteps.
-  Qed.
-  #[local] Lemma owner₁_update γ stable back ws vs :
-    owner₁ γ stable back ws -∗
-    model₁ γ vs -∗
-    model₂ γ vs ==∗
-      owner₁ γ stable back vs ∗
-      model₁ γ vs ∗
-      model₂ γ vs.
-  Proof.
-    iIntros "(:owner₁) Hmodel₁ Hmodel₂".
-    iMod (auth_twins_update_auth with "Hmodel_auth Hmodel₁ Hmodel₂") as "($ & $ & $)".
-    iSteps.
-  Qed.
-  #[local] Lemma owner_update {γ stable1 back1 ws stable2 back2} stable back :
-    owner₁ γ stable1 back1 ws -∗
-    owner₂ γ stable2 back2 ==∗
-      owner₁ γ stable back ws ∗
-      owner₂ γ stable back.
-  Proof.
-    iIntros "(:owner₁) Howner₂".
-    iMod (twins_update with "Howner₁ Howner₂") as "(Howner₁ & Howner₂)".
-    iSteps.
-  Qed.
-
-  #[local] Lemma front_alloc :
-    ⊢ |==>
-      ∃ γ_front,
-      front_auth' γ_front 1.
-  Proof.
-    apply auth_nat_max_alloc.
-  Qed.
-  #[local] Lemma front_lb_get γ front :
-    front_auth γ front ⊢
-    front_lb γ front.
-  Proof.
-    apply auth_nat_max_lb_get.
-  Qed.
-  #[local] Lemma front_lb_le {γ front} front' :
-    front' ≤ front →
-    front_lb γ front ⊢
-    front_lb γ front'.
-  Proof.
-    apply auth_nat_max_lb_le.
-  Qed.
-  #[local] Lemma front_lb_valid γ front1 front2 :
-    front_auth γ front1 -∗
-    front_lb γ front2 -∗
-    ⌜front2 ≤ front1⌝.
-  Proof.
-    apply auth_nat_max_lb_valid.
-  Qed.
-  #[local] Lemma front_update γ front :
-    front_auth γ front ⊢ |==>
-    front_auth γ (S front).
-  Proof.
-    apply auth_nat_max_update; first lia.
-  Qed.
-
-  #[local] Lemma history_alloc :
-    ⊢ |==>
-      ∃ γ_hist,
-      history_auth' γ_hist [()%V].
-  Proof.
-    apply mono_list_alloc.
-  Qed.
-  #[local] Lemma history_at_get {γ hist v} i :
-    i = length hist →
-    history_auth γ (hist ++ [v]) ⊢
-    history_at γ i v.
-  Proof.
-    intros ->.
-    apply mono_list_at_get, list_lookup_middle. done.
-  Qed.
-  #[local] Lemma history_at_lookup γ hist i v :
-    history_auth γ hist -∗
-    history_at γ i v -∗
-    ⌜hist !! i = Some v⌝.
-  Proof.
-    apply mono_list_at_valid.
-  Qed.
-  #[local] Lemma history_at_agree γ i v1 v2 :
-    history_at γ i v1 -∗
-    history_at γ i v2 -∗
-    ⌜v1 = v2⌝.
-  Proof.
-    apply mono_list_at_agree.
-  Qed.
-  #[local] Lemma history_update {γ hist} i v :
-    i = length hist →
-    history_auth γ hist ⊢ |==>
-      history_auth γ (hist ++ [v]) ∗
-      history_at γ i v.
-  Proof.
-    iIntros (->) "Hauth".
-    iMod (mono_list_update_snoc with "Hauth") as "Hauth".
-    iDestruct (history_at_get with "Hauth") as "#Hat"; first done.
-    iSteps.
-  Qed.
-
-  #[local] Lemma winner_alloc :
-    ⊢ |==>
-      ∃ γ_winner,
-      winner_pop' γ_winner 1 True ∗
-      winner_steal' γ_winner 1 True.
-  Proof.
-    apply twins_alloc'.
-  Qed.
-  #[local] Lemma winner_pop_exclusive γ front1 P1 front2 P2 :
-    winner_pop γ front1 P1 -∗
-    winner_pop γ front2 P2 -∗
-    False.
-  Proof.
-    apply twins_twin1_exclusive.
-  Qed.
-  #[local] Lemma winner_pop_exclusive' γ front P :
-    winner_pop γ front P -∗
-    winner γ -∗
-    False.
-  Proof.
-    iIntros "Hwinner_pop_1 (:winner =2)".
-    iApply (winner_pop_exclusive with "Hwinner_pop_1 Hwinner_pop_2").
-  Qed.
-  #[local] Lemma winner_steal_exclusive γ front1 P1 front2 P2 :
-    winner_steal γ front1 P1 -∗
-    winner_steal γ front2 P2 -∗
-    False.
-  Proof.
-    apply twins_twin2_exclusive.
-  Qed.
-  #[local] Lemma winner_steal_exclusive' γ front P :
-    winner_steal γ front P -∗
-    winner γ -∗
-    False.
-  Proof.
-    iIntros "Hwinner_steal_1 (:winner =2)".
-    iApply (winner_steal_exclusive with "Hwinner_steal_1 Hwinner_steal_2").
-  Qed.
-  #[local] Lemma winner_agree γ front1 P1 front2 P2 :
-    winner_pop γ front1 P1 -∗
-    winner_steal γ front2 P2 -∗
-      ⌜front1 = front2⌝ ∗
-      ▷ (P1 ≡ P2).
-  Proof.
-    iIntros "Hwinner_pop Hwinner_steal".
-    iDestruct (twins_agree with "Hwinner_pop Hwinner_steal") as "#Heq".
-    rewrite prod_equivI /= discrete_eq_1.
-    iDestruct "Heq" as "($ & $)".
-  Qed.
-  #[local] Lemma winner_update {γ front1 P1 front2 P2} front P :
-    winner_pop γ front1 P1 -∗
-    winner_steal γ front2 P2 ==∗
-      winner_pop γ front P ∗
-      winner_steal γ front P.
-  Proof.
-    apply twins_update.
-  Qed.
-
-  Opaque owner₁'.
-
   Lemma ws_bdeque_1_model_valid t ι cap vs :
     ws_bdeque_1_inv t ι cap -∗
     ws_bdeque_1_model t vs -∗
     ⌜length vs ≤ cap⌝.
   Proof.
-    iIntros "(:inv) (:model)". injection Heq as <-.
-    iDestruct (meta_agree with "Hmeta Hmeta_") as %<-.
-    iSteps.
+    iIntros "(:inv =1) (:model =2)". simplify.
+    iDestruct (meta_agree with "Hmeta_1 Hmeta_2") as %->.
+    iApply (base.ws_bdeque_1_model_valid with "Hinv_1 Hmodel_2").
   Qed.
   Lemma ws_bdeque_1_model_exclusive t vs1 vs2 :
     ws_bdeque_1_model t vs1 -∗
@@ -813,18 +2235,7 @@ Section ws_bdeque_1_G.
   Proof.
     iIntros "(:model =1) (:model =2)". simplify.
     iDestruct (meta_agree with "Hmeta_1 Hmeta_2") as %->.
-    iApply (model₁_exclusive with "Hmodel₁_1 Hmodel₁_2").
-  Qed.
-
-  #[local] Lemma owner_2_rebase {l γ stable back ws front_cache i1 us} i2 :
-    0 < γ.(metadata_capacity) →
-    owner_2 l γ stable back ws front_cache i1 us ⊢
-      ∃ us,
-      owner_2 l γ stable back ws front_cache i2 us.
-  Proof.
-    iIntros "%Hcapacity (:owner_2)".
-    iDestruct (array_cslice_rebase i2 with "Hdata_cslice₂") as "(%us' & %n & -> & Hdata_cslice₂ & _)"; [done.. |].
-    iSteps. simpl_length.
+    iApply (base.ws_bdeque_1_model_exclusive with "Hmodel_1 Hmodel_2").
   Qed.
 
   Lemma ws_bdeque_1_owner_exclusive t ws1 ws2 :
@@ -832,137 +2243,18 @@ Section ws_bdeque_1_G.
     ws_bdeque_1_owner t ws2 -∗
     False.
   Proof.
-    iIntros "(:owner =1) (:owner =2)". subst t. injection Heq2 as <-.
+    iIntros "(:owner =1) (:owner =2)". simplify.
     iDestruct (meta_agree with "Hmeta_1 Hmeta_2") as %->.
-    iDestruct "Howner_1" as "(:owner_2 =1)".
-    iDestruct "Howner_2" as "(:owner_2 =2)".
-    iApply (owner₁_exclusive with "Howner₁_1 Howner₁_2").
+    iApply (base.ws_bdeque_1_owner_exclusive with "Howner_1 Howner_2").
   Qed.
-  Lemma ws_bdeque_1_owner_model t ws vs :
-    ws_bdeque_1_owner t ws -∗
-    ws_bdeque_1_model t vs -∗
+  Lemma ws_bdeque_1_owner_model γ ws vs :
+    ws_bdeque_1_owner γ ws -∗
+    ws_bdeque_1_model γ vs -∗
     ⌜vs `suffix_of` ws⌝.
   Proof.
     iIntros "(:owner =1) (:model =2)". simplify.
     iDestruct (meta_agree with "Hmeta_1 Hmeta_2") as %->.
-    iDestruct "Howner_1" as "(:owner_2 =1)".
-    iApply (model₁_valid with "Howner₁_1 Hmodel₁_2").
-  Qed.
-
-  #[local] Lemma inv_state_Stable γ state front back hist vs priv prophs :
-    length vs = back - front →
-    inv_state γ state Stable front back hist vs priv prophs ⊢
-      ⌜state = Empty ∨ state = Nonempty⌝ ∗
-      ⌜front ≤ back⌝.
-  Proof.
-    iIntros "%Hvs Hstate".
-    destruct state.
-    - iDestruct "Hstate" as "(:inv_state_empty lazy=)".
-      iSteps.
-    - iDestruct "Hstate" as "(:inv_state_nonempty lazy=)".
-      iSteps.
-    - iDestruct "Hstate" as "(:inv_state_emptyish lazy=)". done.
-    - iDestruct "Hstate" as "(:inv_state_superempty lazy=)". done.
-  Qed.
-  #[local] Lemma inv_state_Unstable γ state front back hist vs priv prophs :
-    inv_state γ state Unstable front back hist vs priv prophs ⊢
-      ⌜state = Emptyish ∨ state = Superempty⌝ ∗
-      ⌜front = back ∨ front = S back⌝.
-  Proof.
-    iIntros "Hstate".
-    destruct state.
-    - iDestruct "Hstate" as "(:inv_state_empty lazy=)". done.
-    - iDestruct "Hstate" as "(:inv_state_nonempty lazy=)". done.
-    - iDestruct "Hstate" as "(:inv_state_emptyish lazy=)".
-      iSteps.
-    - iDestruct "Hstate" as "(:inv_state_superempty lazy=)".
-      iSteps.
-  Qed.
-  #[local] Lemma inv_state_Nonempty γ state stable front back hist vs priv prophs :
-    front < back →
-    inv_state γ state stable front back hist vs priv prophs ⊢
-    ⌜state = Nonempty⌝.
-  Proof.
-    iIntros "% Hstate".
-    destruct state.
-    - iDestruct "Hstate" as "(:inv_state_empty)". lia.
-    - done.
-    - iDestruct "Hstate" as "(:inv_state_emptyish)". lia.
-    - iDestruct "Hstate" as "(:inv_state_superempty)". lia.
-  Qed.
-  #[local] Lemma inv_state_Superempty γ state front back hist vs priv prophs :
-    back < front →
-    inv_state γ state Unstable front back hist vs priv prophs -∗
-    ⌜state = Superempty⌝.
-  Proof.
-    iIntros "% Hstate".
-    destruct state.
-    - iDestruct "Hstate" as "(:inv_state_empty lazy=)". done.
-    - iDestruct "Hstate" as "(:inv_state_nonempty lazy=)". done.
-    - iDestruct "Hstate" as "(:inv_state_emptyish lazy=)". lia.
-    - done.
-  Qed.
-  #[local] Lemma inv_state_winner_pop γ state stable front1 back hist vs priv prophs front2 P :
-    inv_state γ state stable front1 back hist vs priv prophs -∗
-    winner_pop γ front2 P -∗
-      ∃ P_,
-      ⌜front1 = front2⌝ ∗
-      ▷ (P ≡ P_) ∗
-      ( inv_state_nonempty_steal γ state stable front2 back hist vs prophs P_
-      ∨ inv_state_emptyish_steal γ state stable front2 back hist priv P_
-      ) ∗
-      winner_pop γ front2 P.
-  Proof.
-    iIntros "Hstate Hwinner_pop".
-    destruct state.
-    - iDestruct "Hstate" as "(:inv_state_empty)".
-      iDestruct "Hwinner" as "(:winner =3)".
-      iDestruct (winner_pop_exclusive with "Hwinner_pop Hwinner_pop_3") as %[].
-    - iDestruct "Hstate" as "(:inv_state_nonempty)".
-      iDestruct "Hwinner" as "[(:winner =3) | Hwinner]".
-      + iDestruct (winner_pop_exclusive with "Hwinner_pop Hwinner_pop_3") as %[].
-      + destruct prophs as [| id prophs]; first done.
-        iDestruct "Hwinner" as "(:winner_pending_2 =_)".
-        iDestruct (winner_agree with "Hwinner_pop Hwinner_steal") as "#(<- & $)".
-        iSteps.
-    - iDestruct "Hstate" as "(:inv_state_emptyish)".
-      iDestruct "Hwinner" as "[Hwinner_pop_ | (:winner_linearized)]".
-      + iDestruct (winner_pop_exclusive with "Hwinner_pop Hwinner_pop_") as %[].
-      + iDestruct (winner_agree with "Hwinner_pop Hwinner_steal") as "#(<- & $)".
-        iSteps.
-    - iDestruct "Hstate" as "(:inv_state_superempty)".
-      iDestruct "Hwinner" as "(:winner =3)".
-      iDestruct (winner_pop_exclusive with "Hwinner_pop Hwinner_pop_3") as %[].
-  Qed.
-  #[local] Lemma inv_state_winner_steal γ state stable front1 back hist vs priv prophs front2 P :
-    inv_state γ state stable front1 back hist vs priv prophs -∗
-    winner_steal γ front2 P -∗
-      ∃ P_,
-      ⌜front1 = front2⌝ ∗
-      ▷ (P_ ≡ P) ∗
-      inv_state_emptyish_pop γ state stable front2 back hist priv P_ ∗
-      winner_steal γ front2 P.
-  Proof.
-    iIntros "Hstate Hwinner_steal".
-    destruct state.
-    - iDestruct "Hstate" as "(:inv_state_empty)".
-      iDestruct "Hwinner" as "(:winner =3)".
-      iDestruct (winner_steal_exclusive with "Hwinner_steal Hwinner_steal_3") as %[].
-    - iDestruct "Hstate" as "(:inv_state_nonempty)".
-      destruct prophs as [| id prophs].
-      + iDestruct "Hwinner" as "[(:winner =3) | []]".
-        iDestruct (winner_steal_exclusive with "Hwinner_steal Hwinner_steal_3") as %[].
-      + iDestruct "Hwinner" as "[(:winner =3) | (:winner_pending_2 =_ !=)]".
-        * iDestruct (winner_steal_exclusive with "Hwinner_steal Hwinner_steal_3") as %[].
-        * iDestruct (winner_steal_exclusive with "Hwinner_steal Hwinner_steal_") as %[].
-    - iDestruct "Hstate" as "(:inv_state_emptyish)".
-      iDestruct "Hwinner" as "[Hwinner_pop | (:winner_linearized !=)]".
-      + iDestruct (winner_agree with "Hwinner_pop Hwinner_steal") as "#(<- & $)".
-        iSteps.
-      + iDestruct (winner_steal_exclusive with "Hwinner_steal Hwinner_steal_") as %[].
-    - iDestruct "Hstate" as "(:inv_state_superempty)".
-      iDestruct "Hwinner" as "(:winner =3)".
-      iDestruct (winner_steal_exclusive with "Hwinner_steal Hwinner_steal_3") as %[].
+    iApply (base.ws_bdeque_1_owner_model with "Howner_1 Hmodel_2").
   Qed.
 
   Lemma ws_bdeque_1_create_spec ι (cap : Z) :
@@ -980,50 +2272,10 @@ Section ws_bdeque_1_G.
   Proof.
     iIntros "%Hcap %Φ _ HΦ".
 
-    wp_rec.
-
-    wp_apply (prophet_multi_wp_proph with "[//]") as (pid γ_prophet prophss) "Hprophet_model".
-
-    wp_apply (array_unsafe_make_spec with "[//]") as (data) "Hdata_model"; first lia.
-    iDestruct (array_model_to_cslice with "Hdata_model") as "Hdata_cslice".
-    iEval (simpl_length) in "Hdata_cslice".
-    iDestruct (array_cslice_rotation_right_0 1 with "Hdata_cslice") as "Hdata_cslice"; [simpl_length; lia.. |].
-    iEval (rewrite rotation_replicate) in "Hdata_cslice".
-    iDestruct "Hdata_cslice" as "(Hdata_cslice₁ & Hdata_cslice₂)".
-
-    wp_block l as "Hmeta" "(Hl_capacity & Hl_front & Hl_front_cache & Hl_back & Hl_data & Hl_proph & _)".
-    iMod (pointsto_persist with "Hl_capacity") as "#Hl_capacity".
-    iMod (pointsto_persist with "Hl_data") as "#Hl_data".
-    iMod (pointsto_persist with "Hl_proph") as "#Hl_proph".
-
-    iMod model_owner_alloc as "(%γ_model & %γ_owner & Hmodel₁ & Hmodel₂ & Howner₁ & Howner₂)".
-    iMod front_alloc as "(%γ_front & Hfront_auth)".
-    iMod history_alloc as "(%γ_history & Hhist_auth)".
-    iMod winner_alloc as "(%γ_winner & Hwinner_pop & Hwinner_steal)".
-
-    set γ := {|
-      metadata_capacity := ₊cap ;
-      metadata_data := data ;
-      metadata_inv := ι ;
-      metadata_prophet := pid ;
-      metadata_prophet_name := γ_prophet ;
-      metadata_model := γ_model ;
-      metadata_owner := γ_owner ;
-      metadata_front := γ_front ;
-      metadata_history := γ_history ;
-      metadata_winner := γ_winner ;
-    |}.
-    iMod (meta_set γ with "Hmeta") as "#Hmeta"; first done.
-
-    iDestruct (front_lb_get γ with "Hfront_auth") as "#Hfront_lb".
-
-    iApply "HΦ".
-    iSplitR "Hmodel₁ Howner₁ Hl_front_cache Hdata_cslice₂".
-    - iExists l, γ. unshelve iStep 8; first iSteps.
-      iApply inv_alloc.
-      iExists Empty, Stable, 1, 1, [()%V], [], (replicate ₊cap ()%V), (λ _, []), prophss. iFrameSteps.
-      simpl_length.
-    - iSteps. simpl_length.
+    iApply wp_fupd.
+    wp_apply (base.ws_bdeque_1_create_spec with "[//]") as (𝑡 γ) "(Hmeta & Hinv & Hmodel & Howner)"; first done.
+    iMod (meta_set γ with "Hmeta"); first done.
+    iSteps.
   Qed.
 
   Lemma ws_bdeque_1_capacity_spec t ι cap :
@@ -1038,526 +2290,7 @@ Section ws_bdeque_1_G.
   Proof.
     iIntros "%Φ (:inv) HΦ".
 
-    wp_rec. wp_load.
-    iSteps.
-  Qed.
-
-  #[local] Lemma front_spec l γ :
-    {{{
-      inv' l γ
-    }}}
-      (#l).{front}
-    {{{ front,
-      RET #front;
-      front_lb γ front
-    }}}.
-  Proof.
-    iIntros "%Φ (:inv') HΦ".
-
-    iInv "Hinv" as "(:inv_inner)".
-    wp_load.
-    iDestruct (front_lb_get with "Hfront_auth") as "#Hfront_lb_1".
-    iFrameSteps.
-  Qed.
-  #[local] Lemma front_spec_owner_Stable l γ back ws :
-    {{{
-      inv' l γ ∗
-      owner₁ γ Stable back ws
-    }}}
-      (#l).{front}
-    {{{ front,
-      RET #front;
-      owner₁ γ Stable back ws ∗
-      front_lb γ front ∗
-      ⌜front ≤ back⌝
-    }}}.
-  Proof.
-    iIntros "%Φ ((:inv') & Howner₁) HΦ".
-
-    iInv "Hinv" as "(:inv_inner =1)".
-    wp_load.
-    iDestruct (owner_agree with "Howner₁ Howner₂") as %(<- & <-).
-    iDestruct (front_lb_get with "Hfront_auth") as "#Hfront_lb".
-    iDestruct (inv_state_Stable with "Hstate") as "#(_ & %)"; first done.
-    iFrameSteps.
-  Qed.
-  #[local] Lemma front_spec_owner_Unstable l γ back ws :
-    {{{
-      inv' l γ ∗
-      owner₁ γ Unstable back ws
-    }}}
-      (#l).{front}
-    {{{ front,
-      RET #front;
-      owner₁ γ Unstable back ws ∗
-      front_lb γ front ∗
-      ⌜front = back ∨ front = S back⌝
-    }}}.
-  Proof.
-    iIntros "%Φ ((:inv') & Howner₁) HΦ".
-
-    iInv "Hinv" as "(:inv_inner =1)".
-    wp_load.
-    iDestruct (owner_agree with "Howner₁ Howner₂") as %(<- & <-).
-    iDestruct (front_lb_get with "Hfront_auth") as "#Hfront_lb".
-    iDestruct (inv_state_Unstable with "Hstate") as "#(_ & %)".
-    iFrameSteps.
-  Qed.
-  #[local] Lemma front_spec_Superempty l γ back ws front :
-    back < front →
-    {{{
-      inv' l γ ∗
-      owner₁ γ Unstable back ws ∗
-      front_lb γ front
-    }}}
-      (#l).{front}
-    {{{
-      RET #front;
-      owner₁ γ Unstable back ws
-    }}}.
-  Proof.
-    iIntros "% %Φ ((:inv') & Howner₁ & #Hfront_lb) HΦ".
-
-    iInv "Hinv" as "(:inv_inner =1)".
-    wp_load.
-    iDestruct (owner_agree with "Howner₁ Howner₂") as %(<- & <-).
-    iDestruct (front_lb_valid with "Hfront_auth Hfront_lb") as %?.
-    iDestruct (inv_state_Superempty with "Hstate") as %->; first lia.
-    iDestruct "Hstate" as "(:inv_state_superempty =1 lazy=)".
-    iSplitR "Howner₁ HΦ". { iExists Superempty. iFrameSteps. }
-    replace (S back) with front by lia.
-    iSteps.
-  Qed.
-  #[local] Lemma front_spec_winner_steal l γ front P :
-    {{{
-      inv' l γ ∗
-      winner_steal γ front P
-    }}}
-      (#l).{front}
-    {{{
-      RET #front;
-      winner_steal γ front P
-    }}}.
-  Proof.
-    iIntros "%Φ ((:inv') & Hwinner_steal) HΦ".
-
-    iInv "Hinv" as "(:inv_inner =1)".
-    wp_load.
-
-    iAssert ⌜front1 = front⌝%I as %->.
-    { iDestruct (inv_state_winner_steal with "Hstate Hwinner_steal") as "(%P_ & $ & _)". }
-
-    iFrameSteps.
-  Qed.
-
-  #[local] Lemma back_spec l γ stable back ws :
-    {{{
-      inv' l γ ∗
-      owner₁ γ stable back ws
-    }}}
-      (#l).{back}
-    {{{
-      RET #back;
-      owner₁ γ stable back ws
-    }}}.
-  Proof.
-    iIntros "%Φ ((:inv') & Howner₁) HΦ".
-
-    iInv "Hinv" as "(:inv_inner =1)".
-    wp_load.
-    iDestruct (owner_agree with "Howner₁ Howner₂") as "(<- & <-)".
-    iFrameSteps.
-  Qed.
-
-  #[local] Lemma set_back_spec_Superempty l γ back ws front (back' : Z) :
-    back < front →
-    back' = S back →
-    {{{
-      inv' l γ ∗
-      owner₁ γ Unstable back ws ∗
-      front_lb γ front
-    }}}
-      #l <-{back} #back'
-    {{{
-      RET ();
-      owner₁ γ Stable (S back) ws
-    }}}.
-  Proof.
-    iIntros (? ->) "%Φ ((:inv') & Howner₁ & #Hfront_lb) HΦ".
-
-    iInv "Hinv" as "(:inv_inner =1)".
-    wp_store.
-    iDestruct (owner_agree with "Howner₁ Howner₂") as %(<- & <-).
-    iMod (owner_update Stable (S back) with "Howner₁ Howner₂") as "(Howner₁ & Howner₂)".
-    iDestruct (front_lb_valid with "Hfront_auth Hfront_lb") as %?.
-    iDestruct (inv_state_Superempty with "Hstate") as %->; first lia.
-    iDestruct "Hstate" as "(:inv_state_superempty =1 lazy=)".
-    iSplitR "Howner₁ HΦ". { iExists Empty. iFrameSteps. }
-    iSteps.
-  Qed.
-
-  #[local] Lemma array_unsafe_cget_spec_loser l γ i :
-    (0 ≤ i)%Z →
-    {{{
-      inv' l γ
-    }}}
-      array_unsafe_cget γ.(metadata_data) #i
-    {{{ v,
-      RET v;
-      True
-    }}}.
-  Proof.
-    iIntros "%Hi %Φ (:inv') HΦ".
-
-    iApply wp_fupd.
-    awp_apply (array_unsafe_cget_spec_atomic_weak with "[//]") without "HΦ"; first done.
-    iInv "Hinv" as "(:inv_inner)".
-    iAaccIntro with "[$Hdata_cslice₁]".
-    { iPureIntro. simpl_length. }
-    { iIntros "(Hdata_cslice₁ & _) !>". iFrameSteps. }
-    iIntros "Hdata_cslice₁ !>".
-    iSplitL. { iFrameSteps. }
-    iIntros "%v H£ HΦ".
-    iApply (lc_fupd_elim_later with "H£ HΦ [//]").
-  Qed.
-  #[local] Lemma array_unsafe_cget_spec_winner_pop l γ front P v :
-    {{{
-      inv' l γ ∗
-      winner_pop γ front P ∗
-      history_at γ front v
-    }}}
-      array_unsafe_cget γ.(metadata_data) #front
-    {{{
-      RET v;
-      winner_pop γ front P
-    }}}.
-  Proof.
-    iIntros "%Φ ((:inv') & Hwinner_pop & #Hhistory_at) HΦ".
-
-    iApply wp_fupd.
-    awp_apply (array_unsafe_cget_spec_atomic with "[//]") without "HΦ".
-    iInv "Hinv" as "(:inv_inner =1)".
-
-    iAssert (◇ (
-      ⌜front1 = front⌝ ∗
-      ⌜hd inhabitant (vs1 ++ priv1) = v⌝
-    ))%I as "#>(-> & %Hlookup)".
-    { iDestruct (inv_state_winner_pop with "Hstate [$Hwinner_pop]") as "(%P_ & >-> & _ & [(:inv_state_nonempty_steal =1 >) | (:inv_state_emptyish_steal =1 >)] & Hwinner_pop)".
-      - iDestruct (history_at_agree with "Hhistory_at Hhistory_at_front1") as ">->".
-        rewrite hd_app //; first lia.
-      - iDestruct (history_at_agree with "Hhistory_at Hhistory_at_front1") as ">->".
-        assert (length vs1 = 0) as ->%nil_length_inv by lia.
-        iSteps.
-    }
-    apply hd_correct in Hlookup; last (simpl_length; lia).
-    rewrite head_lookup in Hlookup.
-
-    iAaccIntro with "[$Hdata_cslice₁]".
-    { rewrite Nat2Z.id Nat.sub_diag. iSteps. }
-    { iIntros "(_ & _ & Hdata_cslice₁) !>". iFrameSteps. }
-    iIntros "Hdata_cslice₁ !>".
-    iSplitR "Hwinner_pop". { iFrameSteps. }
-    iIntros "H£ HΦ".
-    iApply (lc_fupd_elim_later with "H£ HΦ Hwinner_pop").
-  Qed.
-
-  #[local] Lemma array_unsafe_cset_spec_owner l γ back ws front_cache us front v :
-    back < front + γ.(metadata_capacity) →
-    {{{
-      inv' l γ ∗
-      owner_2 l γ Stable back ws front_cache back us ∗
-      front_lb γ front
-    }}}
-      array_unsafe_cset γ.(metadata_data) #back v
-    {{{
-      RET ();
-      owner_2 l γ Stable back ws front_cache back (<[0 := v]> us)
-    }}}.
-  Proof.
-    iIntros "% %Φ ((:inv') & (:owner_2) & #Hfront_lb) HΦ".
-
-    iApply wp_fupd.
-    awp_apply (array_unsafe_cset_spec_atomic_cell with "[//]") without "HΦ".
-    iInv "Hinv" as "(:inv_inner =1)".
-    iDestruct (owner_agree with "Howner₁ Howner₂") as %(<- & <-).
-    iDestruct (front_lb_valid with "Hfront_auth Hfront_lb") as %?.
-    iDestruct (inv_state_Stable with "Hstate") as "#>(%Hstate1 & %)"; first done.
-
-    iDestruct (array_cslice_app with "Hdata_cslice₁") as "(Hdata_cslice₁_1 & Hdata_cslice₁_2)".
-    destruct (lookup_lt_is_Some_2 priv1 0) as (w & Hpriv_lookup); first lia.
-    iDestruct (array_cslice_update with "Hdata_cslice₁_2") as "(Hdata_back₁ & Hdata_cslice₁_2)"; first done.
-    replace (front1 + length vs1 + 0) with back by lia.
-
-    destruct (lookup_lt_is_Some_2 us 0) as (w_ & Hus_lookup); first lia.
-    iDestruct (array_cslice_update with "Hdata_cslice₂") as "(Hdata_back₂ & Hdata_cslice₂)"; first done.
-    iEval (rewrite Nat.add_0_r) in "Hdata_back₂ Hdata_cslice₂".
-
-    iDestruct (array_cslice_combine with "Hdata_back₁ Hdata_back₂") as "(%Heq & Hdata_back)"; first done. injection Heq as <-.
-    iEval (rewrite dfrac_op_own Qp.half_half) in "Hdata_back".
-
-    iAaccIntro with "[$Hdata_back]". 1: iSteps.
-
-    - iIntros "(_ & (Hdata_back₁ & Hdata_back₂)) !>".
-
-      iDestruct (array_cslice_app_1 with "Hdata_cslice₁_1 (Hdata_cslice₁_2 Hdata_back₁)") as "Hdata_cslice₁"; first done.
-      iEval (rewrite list_insert_id //) in "Hdata_cslice₁".
-
-      iDestruct ("Hdata_cslice₂" with "Hdata_back₂") as "Hdata_cslice₂".
-      iEval (rewrite list_insert_id //) in "Hdata_cslice₂".
-
-      iFrameSteps.
-
-    - iIntros "(Hdata_back₁ & Hdata_back₂) !>".
-
-      iDestruct (array_cslice_app_1 with "Hdata_cslice₁_1 (Hdata_cslice₁_2 Hdata_back₁)") as "Hdata_cslice₁"; first done.
-
-      iDestruct ("Hdata_cslice₂" with "Hdata_back₂") as "Hdata_cslice₂".
-
-      iSplitR "Howner₁ Hl_front_cache Hdata_cslice₂".
-      { iFrameSteps.
-        - iPureIntro. simpl_length.
-        - iExists state1.
-          destruct Hstate1 as [-> | ->]; iFrameSteps.
-      }
-      iIntros "H£ HΦ".
-
-      iMod (lc_fupd_elim_later with "H£ HΦ") as "HΦ".
-      iSteps. iPureIntro. simpl_length.
-  Qed.
-
-  #[local] Lemma resolve_spec_loser_1 l γ front1 front2 id :
-    front1 < front2 →
-    {{{
-      inv' l γ ∗
-      front_lb γ front2
-    }}}
-      Resolve (CAS (#l).[front]%V #front1 #(front1 + 1)) #γ.(metadata_prophet) (#front1, #id)%V
-    {{{
-      RET false;
-      True
-    }}}.
-  Proof.
-    iIntros "%Hloser %Φ ((:inv') & #Hfront_lb) HΦ".
-
-    iInv "Hinv" as "(:inv_inner =3)".
-    iDestruct (front_lb_valid with "Hfront_auth Hfront_lb") as %?.
-    wp_apply (prophet_multi_wp_resolve' with "Hprophet_model"); [done.. |].
-    wp_cas as Hcas; zoo_simplify in Hcas; last lia.
-    iIntros "!> %prophs %Hprophss3 Hprophet_model".
-    iSplitR "HΦ".
-    { iFrameSteps.
-      - iPureIntro => *.
-        rewrite fn_lookup_alter_ne; first lia.
-        auto.
-      - rewrite fn_lookup_insert_ne //. iSteps.
-    }
-    iSteps.
-  Qed.
-  #[local] Lemma resolve_spec_loser_2 l γ front id prophs0 :
-    head prophs0 ≠ Some id →
-    {{{
-      inv' l γ ∗
-      front_lb γ front ∗
-      prophet_multi_full prophet_identifier γ.(metadata_prophet_name) front prophs0
-    }}}
-      Resolve (CAS (#l).[front]%V #front #(front + 1)) #γ.(metadata_prophet) (#front, #id)%V
-    {{{
-      RET false;
-      front_lb γ (S front)
-    }}}.
-  Proof.
-    iIntros "%Hloser %Φ ((:inv') & #Hfront_lb & #Hprophet_full) HΦ".
-
-    iInv "Hinv" as "(:inv_inner =1)".
-    iDestruct (front_lb_valid with "Hfront_auth Hfront_lb") as %?.
-    wp_apply (prophet_multi_wp_resolve' with "Hprophet_model"); [done.. |].
-    wp_apply (wp_cas_nobranch' with "Hl_front") as (b) "%Hcas Hl_front".
-    iIntros "%prophs %Hprophss1 Hprophet_model".
-    destruct b; zoo_simplify in Hcas; first subst front1.
-
-    - iDestruct (prophet_multi_full_valid with "Hprophet_model Hprophet_full") as %->.
-      rewrite fn_lookup_alter Hpasts1 // in Hloser.
-
-    - iDestruct (front_lb_get with "Hfront_auth") as "#-#Hfront_lb_1".
-      iDestruct (front_lb_le (S front) with "Hfront_lb_1") as "-##Hfront_lb_1"; first lia.
-      iSplitR "HΦ".
-      { iFrameSteps.
-        - iPureIntro => *.
-          rewrite fn_lookup_alter_ne; first lia.
-          auto.
-        - rewrite fn_lookup_insert_ne //. iSteps.
-      }
-      iSteps.
-  Qed.
-  #[local] Lemma resolve_spec_winner_pop l γ front P id :
-    {{{
-      inv' l γ ∗
-      winner_pop γ front P
-    }}}
-      Resolve (CAS (#l).[front]%V #front #(front + 1)) #γ.(metadata_prophet) (#front, #id)%V
-    {{{
-      RET true;
-      ▷ P
-    }}}.
-  Proof.
-    iIntros "%Φ ((:inv') & Hwinner_pop) HΦ".
-
-    iInv "Hinv" as "(:inv_inner =1)".
-    wp_apply (prophet_multi_wp_resolve' with "Hprophet_model"); [done.. |].
-    wp_apply (wp_cas_nobranch' with "Hl_front") as (b) "%Hcas Hl_front".
-    iIntros "%prophs %Hprophss1 Hprophet_model".
-    iDestruct (inv_state_winner_pop with "Hstate Hwinner_pop") as "(%P_ & -> & #Heq & Hstate & Hwinner_pop)".
-    rewrite Hprophss1.
-    destruct b; zoo_simplify in Hcas; last congruence.
-    iMod (front_update with "Hfront_auth") as "Hfront_auth".
-    iDestruct "Hstate" as "[(:inv_state_nonempty_steal =1) | (:inv_state_emptyish_steal =1)]".
-
-    - iDestruct "Hwinner" as "(:winner_pending_1)".
-      destruct vs1 as [| v1 vs1] => /=; first naive_solver lia.
-
-      iMod "HP" as "(%vs & Hmodel₁ & _ & HP)".
-      iDestruct (model_agree with "Hmodel₁ Hmodel₂") as %->.
-      iMod (model_steal with "Hmodel₁ Hmodel₂") as "(Hmodel₁ & Hmodel₂) /=".
-      iMod ("HP" with "[$Hmodel₁ $Hhistory_at_front1 //]") as "HP".
-
-      iDestruct (array_cslice_rotation_right_1' (S front) 1 with "Hdata_cslice₁") as "Hdata_cslice₁"; [simpl_length/=; lia.. |].
-      eassert (rotation _ _ = vs1 ++ priv1 ++ [v1]) as ->.
-      { destruct_decide (γ.(metadata_capacity) = 1) as Heq | ?.
-        - rewrite -> Heq in *.
-          simpl in Hdata1.
-          assert (length vs1 = 0) as ->%nil_length_inv by lia.
-          assert (length priv1 = 0) as ->%nil_length_inv by lia.
-          done.
-        - rewrite Nat.mod_1_l; first lia.
-          rewrite rotation_S; first lia.
-          rewrite rotation_0 assoc //.
-      }
-
-      iSplitR "HP HΦ".
-      { destruct_decide (S front = back1) as <- | ?.
-
-        - simpl in Hvs1.
-          iExists Empty. iFrameSteps; iPureIntro.
-          + simpl_length/=. lia.
-          + intros.
-            rewrite fn_lookup_alter_ne; first lia.
-            apply Hpasts1; first lia.
-
-        - destruct vs1 as [| v2 vs1] => /=; first naive_solver lia.
-          simpl in Hvs1.
-          iMod (history_update _ v2 with "Hhistory_auth") as "(Hhistory_auth & #Hhistory_at)"; first done.
-          iExists Nonempty. iFrameSteps; iPureIntro.
-          + simpl_length/=. lia.
-          + intros.
-            rewrite fn_lookup_alter_ne; first lia.
-            apply Hpasts1; first lia.
-          + simpl_length/=. lia.
-      }
-      iIntros "!> {%}".
-
-      iApply "HΦ". iModIntro.
-      iRewrite "Heq" => //.
-
-    - assert (length vs1 = 0) as ->%nil_length_inv by lia.
-
-      iDestruct (array_cslice_rotation_right_1' (S back1) 1 with "Hdata_cslice₁") as "Hdata_cslice₁"; [simpl_length; lia.. |].
-      iEval (rewrite /= -(app_nil_l (rotation _ _))) in "Hdata_cslice₁".
-
-      iSplitR "HP HΦ".
-      { iExists Superempty. iFrameSteps; iPureIntro.
-        - simpl_length.
-        - intros.
-          rewrite fn_lookup_alter_ne; first lia.
-          apply Hpasts1; first lia.
-      }
-      iIntros "!> {%}".
-
-      iApply "HΦ". iModIntro.
-      iRewrite "Heq" => //.
-  Qed.
-  #[local] Lemma resolve_spec_winner_steal l γ front P id :
-    {{{
-      inv' l γ ∗
-      winner_steal γ front P
-    }}}
-      Resolve (CAS (#l).[front]%V #front #(front + 1)) #γ.(metadata_prophet) (#front, #id)%V
-    {{{
-      RET true;
-      front_lb γ (S front)
-    }}}.
-  Proof.
-    iIntros "%Φ ((:inv') & Hwinner_steal) HΦ".
-
-    iInv "Hinv" as "(:inv_inner =1)".
-    wp_apply (prophet_multi_wp_resolve' with "Hprophet_model"); [done.. |].
-    wp_apply (wp_cas_nobranch' with "Hl_front") as (b) "%Hcas Hl_front".
-    iIntros "%prophs %Hprophss1 Hprophet_model".
-    iDestruct (inv_state_winner_steal with "Hstate Hwinner_steal") as "(%P_ & -> & _ & (:inv_state_emptyish_pop =1) & Hwinner_steal)".
-    destruct b; zoo_simplify in Hcas; last congruence.
-    iMod (front_update with "Hfront_auth") as "Hfront_auth".
-    iDestruct (front_lb_get with "Hfront_auth") as "#Hfront_lb".
-
-    assert (length vs1 = 0) as ->%nil_length_inv by lia.
-
-    iDestruct (array_cslice_rotation_right_1' (S back1) 1 with "Hdata_cslice₁") as "Hdata_cslice₁"; [simpl_length; lia.. |].
-    iEval (rewrite /= -(app_nil_l (rotation _ _))) in "Hdata_cslice₁".
-
-    iSplitR "HΦ".
-    { iExists Superempty. iFrameSteps; iPureIntro.
-      - simpl_length.
-      - intros.
-        rewrite fn_lookup_alter_ne; first lia.
-        apply Hpasts1; first lia.
-    }
-    iSteps.
-  Qed.
-  #[local] Lemma resolve_spec_Empty l γ back ws id :
-    {{{
-      inv' l γ ∗
-      owner₁ γ Stable back ws ∗
-      front_lb γ back
-    }}}
-      Resolve (CAS (#l).[front]%V #back #(back + 1)) #γ.(metadata_prophet) (#back, #id)%V
-    {{{
-      RET true;
-      owner₁ γ Unstable back ws ∗
-      front_lb γ (S back)
-    }}}.
-  Proof.
-    iIntros "%Φ ((:inv') & Howner₁ & #Hfront_lb) HΦ".
-
-    iInv "Hinv" as "(:inv_inner =1)".
-    wp_apply (prophet_multi_wp_resolve' with "Hprophet_model"); [done.. |].
-    wp_apply (wp_cas_nobranch' with "Hl_front") as (b) "%Hcas Hl_front".
-    iIntros "%prophs %Hprophss1 Hprophet_model".
-    iDestruct (owner_agree with "Howner₁ Howner₂") as %(<- & <-).
-    iDestruct (front_lb_valid with "Hfront_auth Hfront_lb") as %?.
-    iDestruct (inv_state_Stable with "Hstate") as "#([-> | ->] & _)"; first done.
-
-    - iDestruct "Hstate" as "(:inv_state_empty =1 lazy=)".
-      assert (length vs1 = 0) as ->%nil_length_inv by lia.
-      destruct b; zoo_simplify in Hcas; last lia.
-
-      iMod (front_update with "Hfront_auth") as "Hfront_auth".
-      iClear "Hfront_lb". iDestruct (front_lb_get with "Hfront_auth") as "#Hfront_lb".
-      iMod (history_update _ inhabitant with "Hhistory_auth") as "(Hhistory_auth & _)"; first done.
-      iMod (owner_update Unstable (length hist1) with "Howner₁ Howner₂") as "(Howner₁ & Howner₂)".
-
-      iDestruct (array_cslice_rotation_right_1' (S (length hist1)) 1 with "Hdata_cslice₁") as "Hdata_cslice₁"; [simpl_length; lia.. |].
-      iEval (rewrite -(app_nil_l (rotation _ _ ))) in "Hdata_cslice₁".
-
-      iSplitR "Howner₁ HΦ".
-      { iExists Superempty. iFrameSteps; iPureIntro.
-        - simpl_length.
-        - intros.
-          rewrite fn_lookup_alter_ne; first lia.
-          apply Hpasts1; first lia.
-        - simpl_length/=. lia.
-      }
-      rewrite Hhist1. iSteps.
-
-    - iDestruct "Hstate" as "(:inv_state_nonempty =1 lazy=)".
-      exfalso. lia.
+    wp_apply (base.ws_bdeque_1_capacity_spec with "[$] HΦ").
   Qed.
 
   Lemma ws_bdeque_1_size_spec t ι cap ws :
@@ -1575,32 +2308,14 @@ Section ws_bdeque_1_G.
       ws_bdeque_1_owner t vs
     >>>.
   Proof.
-    iIntros "%Φ ((:inv) & (:owner)) HΦ". injection Heq as <-.
-    iDestruct (meta_agree with "Hmeta Hmeta_") as %<-. iClear "Hmeta_".
-    iDestruct "Howner" as "(:owner_2)".
+    iIntros "%Φ ((:inv =1) & (:owner =2)) HΦ". simplify.
+    iDestruct (meta_agree with "Hmeta_1 Hmeta_2") as %->. iClear "Hmeta_1".
 
-    wp_rec.
-
-    wp_bind (_.{front})%E.
-    iInv "Hinv" as "(:inv_inner =1)".
-    wp_load.
-    iDestruct (owner_agree with "Howner₁ Howner₂") as %(<- & <-).
-    iDestruct (inv_state_Stable with "Hstate") as %(_ & Hback); first done.
-
-    iMod "HΦ" as "(%vs & (:model) & _ & HΦ)". injection Heq as <-.
-    iDestruct (meta_agree with "Hmeta Hmeta_") as %<-. iClear "Hmeta_".
-    iDestruct (model_owner₁_agree with "Howner₁ Hmodel₁ Hmodel₂") as %(Hsuffix & <-).
-    iMod (owner₁_update with "Howner₁ Hmodel₁ Hmodel₂") as "(Howner₁ & Hmodel₁ & Hmodel₂)".
-    iMod ("HΦ" with "[$Hmodel₁]") as "HΦ"; first iSteps.
-
-    iSplitR "Howner₁ Hl_front_cache Hdata_cslice₂ HΦ". { iFrameSteps. }
-    iIntros "!> {%- Hcapacity Hfront_cache Hus Hvs1 Hback}".
-
-    wp_apply (back_spec with "[$Howner₁]") as "Howner₁"; first iSteps.
-    wp_pures.
-
-    replace (⁺back - ⁺front1)%Z with ⁺(length vs) by lia.
-    iSteps.
+    awp_apply (base.ws_bdeque_1_size_spec with "[$]").
+    { iApply (aacc_aupd_commit with "HΦ"); first done. iIntros "%vs (:model =1)". simplify.
+      iDestruct (meta_agree with "Hmeta_1 Hmeta_2") as %<-. iClear "Hmeta_2".
+      iAaccIntro with "Hmodel_1"; iSteps.
+    }
   Qed.
 
   Lemma ws_bdeque_1_is_empty_spec t ι cap ws :
@@ -1618,32 +2333,16 @@ Section ws_bdeque_1_G.
       ws_bdeque_1_owner t vs
     >>>.
   Proof.
-    iIntros "%Φ (#Hinv & Howner) HΦ".
+    iIntros "%Φ ((:inv =1) & (:owner =2)) HΦ". simplify.
+    iDestruct (meta_agree with "Hmeta_1 Hmeta_2") as %->. iClear "Hmeta_1".
 
-    wp_rec.
-    wp_apply (ws_bdeque_1_size_spec with "[$]").
-    iApply (atomic_update_wand with "HΦ"). iIntros "%vs HΦ (%Hvs & Howner)".
-    wp_pures.
-
-    rewrite (bool_decide_ext (⁺(length vs) = 0) (vs = [])).
-    { rewrite -length_zero_iff_nil. lia. }
-    iApply "HΦ".
-    iFrameSteps.
+    awp_apply (base.ws_bdeque_1_is_empty_spec with "[$]").
+    { iApply (aacc_aupd_commit with "HΦ"); first done. iIntros "%vs (:model =1)". simplify.
+      iDestruct (meta_agree with "Hmeta_1 Hmeta_2") as %<-. iClear "Hmeta_2".
+      iAaccIntro with "Hmodel_1"; iSteps.
+    }
   Qed.
 
-  #[local] Definition push_au l γ ws v Φ : iProp Σ :=
-    AU <{
-      ∃∃ vs,
-      ws_bdeque_1_model #l vs
-    }> @ ⊤ ∖ ↑γ.(metadata_inv), ∅ <{
-      ∀∀ b,
-      ⌜b = bool_decide (length vs < γ.(metadata_capacity))⌝ ∗
-      ⌜vs `suffix_of` ws⌝ ∗
-      ws_bdeque_1_model #l (if b then vs ++ [v] else vs)
-    , COMM
-      ws_bdeque_1_owner #l (if b then vs ++ [v] else ws) -∗
-      Φ #b
-    }>.
   Lemma ws_bdeque_1_push_spec t ι cap ws v :
     <<<
       ws_bdeque_1_inv t ι cap ∗
@@ -1661,129 +2360,14 @@ Section ws_bdeque_1_G.
       ws_bdeque_1_owner t (if b then vs ++ [v] else ws)
     >>>.
   Proof.
-    iIntros "%Φ ((:inv) & (:owner)) HΦ". injection Heq as <-.
-    iDestruct (meta_agree with "Hmeta Hmeta_") as %<-. iClear "Hmeta_".
-    rename us into us0. iDestruct (owner_2_rebase back with "Howner") as "(%us & (:owner_2))"; first done.
+    iIntros "%Φ ((:inv =1) & (:owner =2)) HΦ". simplify.
+    iDestruct (meta_agree with "Hmeta_1 Hmeta_2") as %->. iClear "Hmeta_1".
 
-    wp_rec.
-    wp_smart_apply (back_spec with "[$Howner₁]") as "Howner₁"; first iSteps.
-    wp_load.
-    wp_smart_apply (array_size_spec_cslice with "Hdata_cslice₂") as "Hdata_cslice₂".
-    wp_load. wp_pures.
-
-    wp_bind (_ or _)%E.
-    wp_apply (wp_wand (λ res,
-      ∃ b front_cache,
-      ⌜res = #b⌝ ∗
-      l.[front_cache] ↦ #front_cache ∗
-      front_lb γ front_cache ∗
-      owner₁ γ Stable back ws ∗
-      if b then
-        ⌜back < front_cache + γ.(metadata_capacity)⌝ ∗
-        push_au l γ ws v Φ
-      else
-        ⌜back ≤ front_cache + γ.(metadata_capacity)⌝ ∗
-        (ws_bdeque_1_owner #l ws -∗ Φ false%V)
-    )%I with "[Howner₁ Hl_front_cache HΦ]") as (res) "{Hfront_lb_cache} {% front_cache Hfront_cache} (%b & %front_cache & -> & Hl_front_cache & #Hfront_lb_cache & Howner₁ & HΦ)".
-    { case_bool_decide; wp_pures.
-
-      - iStep. iFrame "#∗". iSteps.
-
-      - wp_rec.
-
-        wp_bind (_.{front})%E.
-        wp_apply (wp_wand (λ res,
-          ∃ front,
-          ⌜res = #front⌝ ∗
-          front_lb γ front ∗
-          owner₁ γ Stable back ws ∗
-          if bool_decide (front_cache < front) then
-            ⌜back < front + γ.(metadata_capacity)⌝ ∗
-            push_au l γ ws v Φ
-          else
-            ⌜back ≤ front + γ.(metadata_capacity)⌝ ∗
-            (ws_bdeque_1_owner #l ws -∗ Φ false%V)
-        )%I with "[Howner₁ HΦ]") as (res) "(%front & -> & #Hfront_lb & Howner₁ & HΦ)".
-        { iInv "Hinv" as "(:inv_inner =1)".
-          wp_load.
-          iDestruct (owner_agree with "Howner₁ Howner₂") as %(<- & <-).
-          iDestruct (front_lb_get with "Hfront_auth") as "#$".
-          case_bool_decide. 1: iFrameSteps.
-
-          iMod "HΦ" as "(%vs & (:model) & _ & HΦ)". injection Heq as <-.
-          iDestruct (meta_agree with "Hmeta Hmeta_") as %<-. iClear "Hmeta_".
-          iDestruct (model_owner₁_agree with "Howner₁ Hmodel₁ Hmodel₂") as %(Hsuffix & <-).
-          rewrite bool_decide_eq_false_2; first lia.
-          iMod ("HΦ" with "[Hmodel₁]") as "HΦ"; first iFrameSteps.
-
-          iFrameSteps.
-        }
-
-        wp_store. wp_pures.
-
-        iFrame "#∗". iPureIntro.
-        erewrite bool_decide_ext; [done | lia].
+    awp_apply (base.ws_bdeque_1_push_spec with "[$]").
+    { iApply (aacc_aupd_commit with "HΦ"); first done. iIntros "%vs (:model =1)". simplify.
+      iDestruct (meta_agree with "Hmeta_1 Hmeta_2") as %<-. iClear "Hmeta_2".
+      iAaccIntro with "Hmodel_1"; iSteps.
     }
-
-    destruct b; wp_pures.
-
-    - iDestruct "HΦ" as "(%Hfront_cache & HΦ)".
-
-      wp_apply (array_unsafe_cset_spec_owner with "[$Howner₁ $Hl_front_cache $Hdata_cslice₂]") as "(:owner_2 !=)"; [done | iSteps |].
-      wp_pures.
-
-      wp_bind (_ <-{back} _)%E.
-      iInv "Hinv" as "(:inv_inner =2)".
-      wp_store.
-      iDestruct (owner_agree with "Howner₁ Howner₂") as %(<- & <-).
-      iMod (owner_update Stable (S back) with "Howner₁ Howner₂") as "(Howner₁ & Howner₂)".
-      iDestruct (inv_state_Stable with "Hstate") as "(%Hstate2 & %)"; first done.
-      iDestruct (front_lb_valid with "Hfront_auth Hfront_lb_cache") as %?.
-
-      iAssert ⌜head priv2 = Some v⌝%I as %(priv2' & ->)%head_Some.
-      { iDestruct (array_cslice_rotation_right_small_1' back (length vs2) with "Hdata_cslice₁") as "Hdata_cslice₁"; [simpl_length; lia.. |].
-        rewrite /rotation drop_app_length.
-        rewrite head_lookup -(lookup_app_l _ (take (length vs2) (vs2 ++ priv2))); first lia.
-        iDestruct (array_cslice_agree with "Hdata_cslice₁ Hdata_cslice₂") as %->.
-        { simpl_length. lia. }
-        rewrite list_lookup_insert_eq //; first lia.
-      }
-      iEval (rewrite (assoc _ _ [_])) in "Hdata_cslice₁".
-
-      iMod "HΦ" as "(%vs & (:model) & _ & HΦ)". injection Heq as <-.
-      iDestruct (meta_agree with "Hmeta Hmeta_") as %<-. iClear "Hmeta_".
-      iDestruct (model_owner₁_agree with "Howner₁ Hmodel₁ Hmodel₂") as %(Hsuffix & <-).
-      iMod (model_push v with "Howner₁ Hmodel₁ Hmodel₂") as "(Howner₁ & Hmodel₁ & Hmodel₂)".
-      iMod ("HΦ" $! true with "[$Hmodel₁]") as "HΦ".
-      { iSteps; iPureIntro.
-        - rewrite bool_decide_eq_true_2 //; first lia.
-        - simpl_length/=. lia.
-      }
-
-      iSplitR "Howner₁ Hl_front_cache Hdata_cslice₂ HΦ".
-      { iExists Nonempty.
-        destruct Hstate2 as [-> | ->].
-
-        - iDestruct "Hstate" as "(:inv_state_empty =1 lazy=)".
-          assert (length vs = 0) as ->%nil_length_inv by lia.
-          iMod (history_update back v with "Hhistory_auth") as "(Hhistory_auth & #Hhistory_at)"; first done.
-          iFrameSteps. iPureIntro.
-          simpl_length/=. lia.
-
-        - iDestruct "Hstate" as "(:inv_state_nonempty =1 lazy=)".
-          iFrameSteps; try iPureIntro.
-          + simpl_length/=. lia.
-          + simpl_length/=. lia.
-          + rewrite hd_app //; first lia.
-      }
-      iIntros "!> {%- Hcapacity Hfront_cache Hus}".
-
-      iSteps. iPureIntro. simpl_length.
-
-    - iDestruct "HΦ" as "(%Hfront_cache & HΦ)".
-
-      iApply "HΦ".
-      iFrameSteps.
   Qed.
 
   Lemma ws_bdeque_1_steal_spec t ι cap :
@@ -1801,216 +2385,13 @@ Section ws_bdeque_1_G.
   Proof.
     iIntros "%Φ (:inv) HΦ".
 
-    iLöb as "HLöb".
-
-    wp_rec.
-    wp_apply (wp_id with "[//]") as (id) "Hid".
-    wp_smart_apply front_spec as (front1) "#Hfront_lb_1"; first iSteps.
-    wp_pures.
-
-    wp_bind (_.{back})%E.
-    iInv "Hinv" as "(:inv_inner =2)".
-    wp_load.
-    iDestruct (front_lb_valid with "Hfront_auth Hfront_lb_1") as %?.
-
-    destruct_decide (front1 < back2) as Hbranch1; last first.
-    { assert (length vs2 = 0) as ->%nil_length_inv by lia.
-
-      iMod "HΦ" as "(%vs & (:model) & _ & HΦ)". injection Heq as <-.
-      iDestruct (meta_agree with "Hmeta Hmeta_") as %<-. iClear "Hmeta_".
-      iDestruct (model_agree with "Hmodel₁ Hmodel₂") as %->.
-      iMod ("HΦ" with "[$Hmodel₁] [//]") as "HΦ"; first iSteps.
-
-      iFrameSteps.
+    awp_apply (base.ws_bdeque_1_steal_spec with "[$]").
+    { iApply (aacc_aupd_commit with "HΦ"); first done. iIntros "%vs (:model =1)". simplify.
+      iDestruct (meta_agree with "Hmeta Hmeta_1") as %->. iClear "Hmeta".
+      iAaccIntro with "Hmodel_1"; iSteps.
     }
-
-    destruct_decide (front1 = front2) as <- | ?; last first.
-    { assert (front1 < front2) as Hbranch2 by lia.
-      iDestruct (front_lb_get with "Hfront_auth") as "#Hfront_lb_2".
-      iSplitR "HΦ". { iFrameSteps. }
-      iIntros "!> {%- Hcapacity Hbranch1 Hbranch2}".
-
-      wp_pures.
-      rewrite bool_decide_eq_false_2; first lia.
-      wp_load.
-      wp_smart_apply array_unsafe_cget_spec_loser as (v) "_"; [lia | iSteps |].
-      wp_load.
-      wp_smart_apply resolve_spec_loser_1; [done | iSteps |].
-      iSteps.
-    }
-
-    iDestruct (prophet_multi_full_get _ front1 with "Hprophet_model") as "#Hprophet_full".
-    iEval (rewrite Hpasts2 //=) in "Hprophet_full".
-
-    destruct_decide (head $ prophss2 front1 = Some id) as (prophs0 & Hbranch3)%head_Some | Hbranch3; last first.
-    { iSplitR "HΦ". { iFrameSteps. }
-      remember (prophss2 front1) as prophs0.
-      iIntros "!> {%- Hcapacity Hbranch1 Hbranch3}".
-
-      wp_pures.
-      rewrite bool_decide_eq_false_2; first lia.
-      wp_load.
-      wp_smart_apply array_unsafe_cget_spec_loser as (v) "_"; [lia | iSteps |].
-      wp_load.
-      wp_smart_apply resolve_spec_loser_2; [done | iSteps |].
-      iSteps.
-    }
-    rewrite Hbranch3.
-
-    iDestruct (inv_state_Nonempty with "Hstate") as %->; first done.
-    iDestruct "Hstate" as "(:inv_state_nonempty =2)".
-    iDestruct "Hwinner" as "[(:winner) | (:winner_pending_2 !=)]"; last first.
-    { iDestruct (identifier_model_exclusive with "Hid Hid_") as %[]. }
-
-    destruct vs2 as [| v vs2] => /=; first naive_solver lia.
-    iMod (winner_update front1 (Φ (Some v)) with "Hwinner_pop Hwinner_steal") as "(Hwinner_pop & Hwinner_steal)".
-
-    iSplitR "Hwinner_pop".
-    { iExists Nonempty. iFrameSteps.
-      rewrite Hbranch3 /winner_pending_2. iSteps. iIntros "!> !>".
-      rewrite /winner_au. iAuIntro.
-      iApply (aacc_aupd_commit with "HΦ"); first done. iIntros "%vs (:model)". injection Heq as <-.
-      iDestruct (meta_agree with "Hmeta Hmeta_") as %<-. iClear "Hmeta_".
-      iAaccIntro with "Hmodel₁"; first iSteps. iIntros "%v_ %vs' (-> & Hmodel₁ & Hhistory_at) !>".
-      iDestruct (history_at_agree with "Hhistory_at Hhistory_at_front2") as %<-.
-      simpl in Hvs. iSteps.
-    }
-    iIntros "!> {%- Hcapacity Hbranch1}".
-
-    wp_pures.
-    rewrite bool_decide_eq_false_2; first lia.
-    wp_load.
-    wp_smart_apply (array_unsafe_cget_spec_winner_pop with "[$Hwinner_pop]") as "Hwinner_pop"; first iSteps.
-    wp_load.
-    wp_smart_apply (resolve_spec_winner_pop with "[$Hwinner_pop]") as "HΦ"; first iSteps.
-    iSteps.
   Qed.
 
-  Inductive pop_state :=
-    | PopNonempty v
-    | PopEmptyishWinner v
-    | PopEmptyishLoser
-    | PopSuperempty.
-  #[local] Lemma ws_bdeque_1_pop_0_spec {l γ} (state : pop_state) {stable} back ws front_cache us id (back_ : Z) :
-    back_ = back →
-    {{{
-      inv' l γ ∗
-      owner_1 OwnerPop l γ stable back ws front_cache back us ∗
-      match state with
-      | PopNonempty v =>
-          ⌜stable = Stable⌝ ∗
-          ⌜us !! 0 = Some v⌝
-      | PopEmptyishWinner v =>
-          ⌜stable = Unstable⌝ ∗
-          ⌜us !! 0 = Some v⌝ ∗
-          winner_steal γ back inhabitant
-      | PopEmptyishLoser =>
-          ∃ id_winner prophs,
-          ⌜stable = Unstable⌝ ∗
-          prophet_multi_full prophet_identifier γ.(metadata_prophet_name) back (id_winner :: prophs) ∗
-          ⌜head (id_winner :: prophs) ≠ Some id⌝
-      | PopSuperempty =>
-          ∃ front,
-          ⌜stable = Unstable⌝ ∗
-          front_lb γ front ∗
-          ⌜front = S back⌝
-      end
-    }}}
-      ws_bdeque_1_pop_0 #l #id #back_
-    {{{ o back front_cache i us,
-      RET o;
-      owner_2 l γ Stable back ws front_cache i us ∗
-      match state with
-      | PopNonempty v =>
-          ⌜o = Some v⌝
-      | PopEmptyishWinner v =>
-          ⌜o = Some v⌝
-      | PopEmptyishLoser =>
-          ⌜o = None⌝
-      | PopSuperempty =>
-          ⌜o = None⌝
-      end
-    }}}.
-  Proof.
-    iIntros (->) "%Φ ((:inv') & (:owner_1) & H) HΦ".
-
-    wp_rec. wp_pures.
-    destruct state.
-
-    - iDestruct "H" as "(-> & %Hus_lookup)".
-      iSpecialize ("HΦ" $! (Some v)).
-
-      wp_apply (front_spec_owner_Stable with "[$Howner₁]") as (front2) "(Howner₁ & #Hfront_lb & %Hfront2)"; first iSteps.
-      wp_pures.
-      rewrite bool_decide_eq_false_2; first lia.
-      wp_pures.
-      case_bool_decide as Hbranch; wp_pures.
-
-      + wp_load.
-        wp_apply (array_unsafe_cget_spec with "Hdata_cslice₂"); [done.. | lia |].
-        iSteps.
-
-      + replace front2 with back by lia.
-
-        wp_store. wp_load.
-        wp_smart_apply (resolve_spec_Empty with "[$Howner₁]") as "{Hfront_lb} (Howner₁ & #Hfront_lb)"; first iSteps.
-        wp_smart_apply (set_back_spec_Superempty with "[$Howner₁ $Hfront_lb]") as "Howner₁"; [lia.. | iSteps |].
-        wp_load.
-        wp_apply (array_unsafe_cget_spec with "Hdata_cslice₂") as "Hdata_cslice₂"; [done.. | lia |].
-        wp_pures.
-
-        iApply "HΦ".
-        iFrame "#∗". iSteps.
-
-    - iDestruct "H" as "(-> & %Hus_lookup & Hwinner_steal)".
-      iSpecialize ("HΦ" $! (Some v)).
-
-      wp_apply (front_spec_winner_steal with "[$Hwinner_steal]") as "Hwinner_steal"; first iSteps.
-      wp_pures.
-      rewrite bool_decide_eq_false_2; first lia.
-      wp_pures.
-      rewrite bool_decide_eq_false_2; first lia.
-      wp_store. wp_load.
-      wp_smart_apply (resolve_spec_winner_steal with "[$Hwinner_steal]") as "#Hfront_lb"; first iSteps.
-      wp_smart_apply (set_back_spec_Superempty with "[$Howner₁ $Hfront_lb]") as "Howner₁"; [lia.. | iSteps |].
-      wp_load.
-      wp_apply (array_unsafe_cget_spec with "Hdata_cslice₂") as "Hdata_cslice₂"; [done.. | lia |].
-      wp_pures.
-
-      iApply "HΦ".
-      iFrame "#∗". iSteps.
-
-    - iDestruct "H" as "(%id_winner & %prophs & -> & #Hprophet_full & %Hloser)".
-      iSpecialize ("HΦ" $! None).
-
-      wp_apply (front_spec_owner_Unstable with "[$Howner₁]") as (front2) "(Howner₁ & #Hfront_lb & %Hbranch)"; first iSteps.
-      wp_pures.
-      destruct Hbranch as [-> | ->].
-
-      + rewrite bool_decide_eq_false_2; first lia.
-        wp_pures.
-        rewrite bool_decide_eq_false_2; first lia.
-        wp_store. wp_load.
-        wp_smart_apply (resolve_spec_loser_2 with "[$Hfront_lb $Hprophet_full]") as "{Hfront_lb} #Hfront_lb"; [done | iSteps |].
-        wp_smart_apply (set_back_spec_Superempty with "[$Howner₁ $Hfront_lb]") as "Howner₁"; [lia.. | iSteps |].
-        wp_pures.
-
-        iApply "HΦ".
-        iFrame "#∗". iSteps.
-
-      + rewrite bool_decide_eq_true_2; first lia.
-        wp_smart_apply (set_back_spec_Superempty with "[$Howner₁ $Hfront_lb]") as "Howner₁"; [lia.. | iSteps |].
-        iSteps.
-
-    - iDestruct "H" as "(%front & -> & #Hfront_lb & ->)".
-      iSpecialize ("HΦ" $! None).
-
-      wp_apply (front_spec_Superempty with "[$Howner₁ $Hfront_lb]") as "Howner₁"; [lia | iSteps |].
-      wp_pures.
-      rewrite bool_decide_eq_true_2; first lia.
-      wp_smart_apply (set_back_spec_Superempty with "[$Howner₁ $Hfront_lb]") as "Howner₁"; [lia.. | iSteps |].
-      iSteps.
-  Qed.
   Lemma ws_bdeque_1_pop_spec t ι cap ws :
     <<<
       ws_bdeque_1_inv t ι cap ∗
@@ -2037,153 +2418,19 @@ Section ws_bdeque_1_G.
       ws_bdeque_1_owner t ws'
     >>>.
   Proof.
-    iIntros "%Φ ((:inv) & (:owner)) HΦ". injection Heq as <-.
-    iDestruct (meta_agree with "Hmeta Hmeta_") as %<-. iClear "Hmeta_".
-    rename us into us0. iDestruct (owner_2_rebase (back - 1) with "Howner") as "(%us & (:owner_2))"; first done.
+    iIntros "%Φ ((:inv =1) & (:owner =2)) HΦ". simplify.
+    iDestruct (meta_agree with "Hmeta_1 Hmeta_2") as %->. iClear "Hmeta_1".
 
-    wp_rec.
-    wp_apply (wp_id with "[//]") as (id) "Hid".
-    wp_smart_apply (back_spec with "[$Howner₁]") as "Howner₁"; first iSteps.
-    wp_pures.
-
-    wp_bind (_ <-{back} _)%E.
-    iInv "Hinv" as "(:inv_inner =1)".
-    wp_store.
-    iDestruct (owner_agree with "Howner₁ Howner₂") as %(<- & <-).
-    iDestruct (inv_state_Stable with "Hstate") as "#(%Hstate1 & %)"; first done.
-    destruct Hstate1 as [-> | ->].
-
-    { iDestruct "Hstate" as "(:inv_state_empty =1 lazy=)".
-      assert (0 < back) as Hback by lia.
-      assert (length vs1 = 0) as ->%nil_length_inv by lia.
-
-      iDestruct (front_lb_get with "Hfront_auth") as "#Hfront_lb".
-      iMod (owner_update Unstable (back - 1) with "Howner₁ Howner₂") as "(Howner₁ & Howner₂)".
-
-      iMod "HΦ" as "(%vs & (:model) & _ & HΦ)". injection Heq as <-.
-      iDestruct (meta_agree with "Hmeta Hmeta_") as %<-. iClear "Hmeta_".
-      iDestruct (model_owner₁_agree with "Howner₁ Hmodel₁ Hmodel₂") as %(Hsuffix & ->).
-      iMod (model_empty with "Howner₁ Hmodel₁ Hmodel₂") as "(Howner₁ & Hmodel₁ & Hmodel₂)".
-      iMod ("HΦ" $! None with "[$Hmodel₁]") as "HΦ"; first iSteps.
-
-      iSplitR "Howner₁ Hl_front_cache Hdata_cslice₂ HΦ".
-      { iExists Superempty. iFrameSteps. }
-      iIntros "!> {%- Hcapacity Hfront_cache Hus Hback}".
-
-      wp_smart_apply (ws_bdeque_1_pop_0_spec PopSuperempty (back - 1) with "[- HΦ]"); [lia | iFrameSteps |].
-      iSteps.
+    awp_apply (base.ws_bdeque_1_pop_spec with "[$]").
+    { iApply (aacc_aupd_commit with "HΦ"); first done. iIntros "%vs (:model =1)". simplify.
+      iDestruct (meta_agree with "Hmeta_1 Hmeta_2") as %<-. iClear "Hmeta_2".
+      iAaccIntro with "Hmodel_1". 1: iSteps. iIntros "%o %ws' ($ & Ho)".
+      iExists o, ws'. destruct o.
+      all: iDecompose "Ho".
+      all: iFrameSteps.
     }
-
-    iDestruct "Hstate" as "(:inv_state_nonempty =1 lazy=)".
-    assert (0 < back) as Hback by lia.
-    destruct vs1 as [| v vs1 _] using rev_ind; first naive_solver lia.
-    simpl_length/= in Hvs1.
-    simpl_length/= in Hdata1.
-
-    destruct_decide (S front1 = back) as <- | Hbranch1.
-
-    - assert (length vs1 = 0) as ->%nil_length_inv.
-      { simpl_length/= in Hvs1. lia. }
-      simpl in *.
-      iEval (rewrite Nat.sub_0_r) in "Hdata_cslice₂".
-
-      iAssert ⌜us !! 0 = Some v⌝%I as %Hus_lookup.
-      { iDestruct (array_cslice_agree with "Hdata_cslice₁ Hdata_cslice₂") as %<-; first (simpl; lia).
-        iSteps.
-      }
-
-      iMod (owner_update Unstable front1 with "Howner₁ Howner₂") as "(Howner₁ & Howner₂)".
-
-      destruct_decide (head $ prophss1 front1 = Some id) as (prophs0 & Hprophss1)%head_Some | Hbranch2.
-
-      + rewrite Hprophss1.
-        iDestruct "Hwinner" as "[(:winner) | (:winner_pending_2 !=)]"; last first.
-        { iDestruct (identifier_model_exclusive with "Hid Hid_") as %[]. }
-        iMod (winner_update front1 inhabitant with "Hwinner_pop Hwinner_steal") as "(Hwinner_pop & Hwinner_steal)".
-
-        iMod "HΦ" as "(%vs & (:model) & _ & HΦ)". injection Heq as <-.
-        iDestruct (meta_agree with "Hmeta Hmeta_") as %<-. iClear "Hmeta_".
-        iDestruct (model_owner₁_agree with "Howner₁ Hmodel₁ Hmodel₂") as %(Hsuffix & ->).
-        iMod (model_pop with "Howner₁ Hmodel₁ Hmodel₂") as "(Howner₁ & Hmodel₁ & Hmodel₂) /=".
-        iMod ("HΦ" $! (Some v) with "[$Hmodel₁]") as "HΦ"; first iSteps.
-
-        iSplitR "Howner₁ Hl_front_cache Hdata_cslice₂ Hwinner_steal HΦ".
-        { iExists Emptyish. iFrameSteps. }
-        iIntros "!> {%- Hcapacity Hfront_cache Hus Hback Hus_lookup}".
-
-        wp_smart_apply (ws_bdeque_1_pop_0_spec (PopEmptyishWinner v) front1 with "[- HΦ]"); [lia | iFrameSteps |].
-        iSteps.
-
-      + iDestruct "Hwinner" as "[(:winner) | Hwinner]".
-
-        { iMod (winner_update front1 inhabitant with "Hwinner_pop Hwinner_steal") as "(Hwinner_pop & Hwinner_steal)".
-
-          iMod "HΦ" as "(%vs & (:model) & _ & HΦ)". injection Heq as <-.
-          iDestruct (meta_agree with "Hmeta Hmeta_") as %<-. iClear "Hmeta_".
-          iDestruct (model_owner₁_agree with "Howner₁ Hmodel₁ Hmodel₂") as %(Hsuffix & ->).
-          iMod (model_pop with "Howner₁ Hmodel₁ Hmodel₂") as "(Howner₁ & Hmodel₁ & Hmodel₂) /=".
-          iMod ("HΦ" $! (Some v) with "[$Hmodel₁]") as "HΦ"; first iSteps.
-
-          iSplitR "Howner₁ Hl_front_cache Hdata_cslice₂ Hwinner_steal HΦ".
-          { iExists Emptyish. iFrameSteps. }
-          iIntros "!> {%- Hcapacity Hfront_cache Hus Hus_lookup}".
-
-          wp_smart_apply (ws_bdeque_1_pop_0_spec (PopEmptyishWinner v) front1 with "[- HΦ]"); [lia | iFrameSteps |].
-          iSteps.
-        }
-
-        iDestruct (prophet_multi_full_get _ front1 with "Hprophet_model") as "#Hprophet_full".
-        iEval (rewrite Hpasts1 //=) in "Hprophet_full".
-        destruct (prophss1 front1) as [| id_winner prophs]; first done.
-        iDestruct "Hwinner" as "(:winner_pending_2 !=)".
-
-        iMod "HP" as "(%vs & Hmodel₁ & _ & HP)".
-        iDestruct (model_agree with "Hmodel₁ Hmodel₂") as %->.
-        iMod (model_steal with "Hmodel₁ Hmodel₂") as "(Hmodel₁ & Hmodel₂) /=".
-        iMod ("HP" with "[$Hmodel₁]") as "HP"; first iSteps.
-
-        iMod "HΦ" as "(%vs & (:model) & _ & HΦ)". injection Heq as <-.
-        iDestruct (meta_agree with "Hmeta Hmeta_") as %<-. iClear "Hmeta_".
-        iDestruct (model_owner₁_agree with "Howner₁ Hmodel₁ Hmodel₂") as %(Hsuffix & ->).
-        iMod (model_empty with "Howner₁ Hmodel₁ Hmodel₂") as "(Howner₁ & Hmodel₁ & Hmodel₂)".
-        iMod ("HΦ" $! None with "[$Hmodel₁]") as "HΦ"; first iSteps.
-
-        iSplitR "Howner₁ Hl_front_cache Hdata_cslice₂ HΦ".
-        { iExists Emptyish. iFrameStep 7. iExists P. iSteps. }
-        iIntros "!> {%- Hcapacity Hfront_cache Hus Hbranch2}".
-
-        wp_smart_apply (ws_bdeque_1_pop_0_spec PopEmptyishLoser front1 with "[- HΦ]"); [lia | iFrameSteps |].
-        iSteps.
-
-    - iMod (owner_update Stable (back - 1) with "Howner₁ Howner₂") as "(Howner₁ & Howner₂)".
-      iEval (rewrite -assoc) in "Hdata_cslice₁".
-
-      iMod "HΦ" as "(%vs & (:model) & _ & HΦ)". injection Heq as <-.
-      iDestruct (meta_agree with "Hmeta Hmeta_") as %<-. iClear "Hmeta_".
-      iDestruct (model_owner₁_agree with "Howner₁ Hmodel₁ Hmodel₂") as %(Hsuffix & ->).
-      iMod (model_pop' with "Howner₁ Hmodel₁ Hmodel₂") as "(Howner₁ & Hmodel₁ & Hmodel₂)".
-      iMod ("HΦ" $! (Some v) with "[$Hmodel₁]") as "HΦ"; first iSteps.
-
-      iAssert ⌜us !! 0 = Some v⌝%I as %Hus_lookup.
-      { iDestruct (array_cslice_rotation_right_small_1' (back - 1) (length vs1) with "Hdata_cslice₁") as "Hdata_cslice₁"; [simpl_length/=; lia.. |].
-        iDestruct (array_cslice_agree with "Hdata_cslice₁ Hdata_cslice₂") as %<-.
-        { simpl_length/=. lia. }
-        rewrite /rotation drop_app_length //.
-      }
-
-      iSplitR "Howner₁ Hl_front_cache Hdata_cslice₂ HΦ".
-      { iExists Nonempty. iFrameSteps.
-        rewrite hd_app //; first lia.
-      }
-      iIntros "!> {%- Hcapacity Hfront_cache Hus Hback Hus_lookup}".
-
-      wp_smart_apply (ws_bdeque_1_pop_0_spec (PopNonempty v) (back - 1) with "[- HΦ]"); [lia | iFrameSteps |].
-      iSteps.
   Qed.
 End ws_bdeque_1_G.
-
-From zoo_saturn Require
-  ws_bdeque_1__opaque.
 
 #[global] Opaque ws_bdeque_1_inv.
 #[global] Opaque ws_bdeque_1_model.
